<?xml version="1.0"?>
<rdf:RDF xmlns="https://w3id.org/def/vaeontology_montes_sierra#"
     xml:base="https://w3id.org/def/vaeontology_montes_sierra"
     xmlns:dc="http://purl.org/dc/elements/1.1/"
     xmlns:bhv="https://w3id.org/spice/SON/SchwartzValues#"
     xmlns:dul="http://www.ontologydesignpatterns.org/ont/dul/DUL.owl#"
     xmlns:mod="https://w3id.org/mod#"
     xmlns:obo="http://purl.obolibrary.org/obo/"
     xmlns:owl="http://www.w3.org/2002/07/owl#"
     xmlns:rdf="http://www.w3.org/1999/02/22-rdf-syntax-ns#"
     xmlns:vae="https://w3id.org/def/vaeontology#"
     xmlns:xml="http://www.w3.org/XML/1998/namespace"
     xmlns:xsd="http://www.w3.org/2001/XMLSchema#"
     xmlns:odrl="http://www.w3.org/ns/odrl/2/"
     xmlns:rdfs="http://www.w3.org/2000/01/rdf-schema#"
     xmlns:skos="http://www.w3.org/2004/02/skos/core#"
     xmlns:vann="http://purl.org/vocab/vann/"
     xmlns:vcvf="http://www.ontologydesignpatterns.org/ont/values/valuecore_with_value_frames.owl#"
     xmlns:swrla="http://swrl.stanford.edu/ontologies/3.3/swrla.owl#"
     xmlns:terms="http://purl.org/dc/terms/"
     xmlns:oboInOwl="http://www.geneontology.org/formats/oboInOwl#">
    <owl:Ontology rdf:about="https://w3id.org/def/vaeontology_montes_sierra">
        <owl:versionIRI rdf:resource="https://w3id.org/def/vaeontology_montes_sierra"/>
        <owl:imports rdf:resource="https://w3id.org/def/vaeontology"/>
        <dc:creator>Andrés Holgado Sánchez - https://orcid.org/my-orcid?orcid=0000-0001-8853-1022</dc:creator>
        <dc:description>Extension of the VAE ontology, an ontology for Value Awareness Engineering: representation and reasoning with human values, modelling the research proposal by: Montes, N., Sierra, C.: Synthesis and properties of optimally value-aligned normative systems. Journal of Artificial Intelligence Research 74, 1739–1774 (2022).
https://doi.org/10.1613/jair.1.13487</dc:description>
        <dc:title>Ontology on &quot;Synthesis and properties of optimally value-aligned normative systems&quot;, Montes, N., Sierra, C. (2022).</dc:title>
        <terms:license>https://creativecommons.org/licenses/by/4.0/</terms:license>
        <vann:preferredNamespacePrefix>vaems</vann:preferredNamespacePrefix>
        <rdfs:comment>Montes, N., Sierra, C.: Synthesis and properties of optimally value-aligned normative systems. Journal of Artificial Intelligence Research 74, 1739–1774 (2022).
https://doi.org/10.1613/jair.1.13487</rdfs:comment>
        <rdfs:seeAlso>https://doi.org/10.1613/jair.1.13487</rdfs:seeAlso>
        <owl:versionInfo>1.0.0</owl:versionInfo>
        <bhv:bibRef>Montes, N., Sierra, C.: Synthesis and properties of optimally value-aligned normative systems. Journal of Artificial Intelligence Research 74, 1739–1774 (2022).
https://doi.org/10.1613/jair.1.13487</bhv:bibRef>
    </owl:Ontology>
    


    <!-- 
    ///////////////////////////////////////////////////////////////////////////////////////
    //
    // Annotation properties
    //
    ///////////////////////////////////////////////////////////////////////////////////////
     -->

    


    <!-- http://purl.org/dc/elements/1.1/creator -->

    <owl:AnnotationProperty rdf:about="http://purl.org/dc/elements/1.1/creator"/>
    


    <!-- http://purl.org/dc/elements/1.1/description -->

    <owl:AnnotationProperty rdf:about="http://purl.org/dc/elements/1.1/description"/>
    


    <!-- http://purl.org/dc/elements/1.1/title -->

    <owl:AnnotationProperty rdf:about="http://purl.org/dc/elements/1.1/title"/>
    


    <!-- http://purl.org/dc/terms/license -->

    <owl:AnnotationProperty rdf:about="http://purl.org/dc/terms/license"/>
    


    <!-- http://purl.org/vocab/vann/preferredNamespacePrefix -->

    <owl:AnnotationProperty rdf:about="http://purl.org/vocab/vann/preferredNamespacePrefix"/>
    


    <!-- http://www.w3.org/2002/07/owl#minQualifiedCardinality -->

    <owl:AnnotationProperty rdf:about="http://www.w3.org/2002/07/owl#minQualifiedCardinality"/>
    


    <!-- http://www.w3.org/2004/02/skos/core#definition -->

    <owl:AnnotationProperty rdf:about="http://www.w3.org/2004/02/skos/core#definition"/>
    


    <!-- https://w3id.org/spice/SON/SchwartzValues#bibRef -->

    <owl:AnnotationProperty rdf:about="https://w3id.org/spice/SON/SchwartzValues#bibRef"/>
    


    <!-- 
    ///////////////////////////////////////////////////////////////////////////////////////
    //
    // Object Properties
    //
    ///////////////////////////////////////////////////////////////////////////////////////
     -->

    


    <!-- http://www.ontologydesignpatterns.org/ont/dul/DUL.owl#associatedWith -->

    <owl:ObjectProperty rdf:about="http://www.ontologydesignpatterns.org/ont/dul/DUL.owl#associatedWith"/>
    


    <!-- http://www.ontologydesignpatterns.org/ont/dul/DUL.owl#classifies -->

    <owl:ObjectProperty rdf:about="http://www.ontologydesignpatterns.org/ont/dul/DUL.owl#classifies"/>
    


    <!-- http://www.ontologydesignpatterns.org/ont/dul/DUL.owl#hasConstituent -->

    <owl:ObjectProperty rdf:about="http://www.ontologydesignpatterns.org/ont/dul/DUL.owl#hasConstituent"/>
    


    <!-- http://www.ontologydesignpatterns.org/ont/dul/DUL.owl#hasConstraint -->

    <owl:ObjectProperty rdf:about="http://www.ontologydesignpatterns.org/ont/dul/DUL.owl#hasConstraint">
        <rdfs:range rdf:resource="http://www.ontologydesignpatterns.org/ont/dul/DUL.owl#Parameter"/>
    </owl:ObjectProperty>
    


    <!-- http://www.ontologydesignpatterns.org/ont/dul/DUL.owl#hasParameter -->

    <owl:ObjectProperty rdf:about="http://www.ontologydesignpatterns.org/ont/dul/DUL.owl#hasParameter">
        <rdfs:subPropertyOf rdf:resource="http://www.ontologydesignpatterns.org/ont/dul/DUL.owl#isRelatedToConcept"/>
        <owl:inverseOf rdf:resource="http://www.ontologydesignpatterns.org/ont/dul/DUL.owl#isParameterFor"/>
        <rdfs:domain rdf:resource="http://www.ontologydesignpatterns.org/ont/dul/DUL.owl#Concept"/>
        <rdfs:range rdf:resource="http://www.ontologydesignpatterns.org/ont/dul/DUL.owl#Parameter"/>
        <rdfs:comment>A Concept can have a Parameter that constrains the attributes that a classified Entity can have in a certain Situation, e.g. a 4WheelDriver Role definedIn the ItalianTrafficLaw has a MinimumAge parameter on the Amount 16.</rdfs:comment>
        <rdfs:isDefinedBy rdf:resource="http://www.ontologydesignpatterns.org/ont/dul/DUL.owl"/>
        <rdfs:label xml:lang="it">ha parametro</rdfs:label>
        <rdfs:label xml:lang="en">has parameter</rdfs:label>
    </owl:ObjectProperty>
    


    <!-- http://www.ontologydesignpatterns.org/ont/dul/DUL.owl#hasPart -->

    <owl:ObjectProperty rdf:about="http://www.ontologydesignpatterns.org/ont/dul/DUL.owl#hasPart"/>
    


    <!-- http://www.ontologydesignpatterns.org/ont/dul/DUL.owl#hasParticipant -->

    <owl:ObjectProperty rdf:about="http://www.ontologydesignpatterns.org/ont/dul/DUL.owl#hasParticipant"/>
    


    <!-- http://www.ontologydesignpatterns.org/ont/dul/DUL.owl#hasSetting -->

    <owl:ObjectProperty rdf:about="http://www.ontologydesignpatterns.org/ont/dul/DUL.owl#hasSetting"/>
    


    <!-- http://www.ontologydesignpatterns.org/ont/dul/DUL.owl#isConstituentOf -->

    <owl:ObjectProperty rdf:about="http://www.ontologydesignpatterns.org/ont/dul/DUL.owl#isConstituentOf"/>
    


    <!-- http://www.ontologydesignpatterns.org/ont/dul/DUL.owl#isConstraintFor -->

    <owl:ObjectProperty rdf:about="http://www.ontologydesignpatterns.org/ont/dul/DUL.owl#isConstraintFor">
        <rdfs:domain rdf:resource="http://www.ontologydesignpatterns.org/ont/dul/DUL.owl#Parameter"/>
    </owl:ObjectProperty>
    


    <!-- http://www.ontologydesignpatterns.org/ont/dul/DUL.owl#isMemberOf -->

    <owl:ObjectProperty rdf:about="http://www.ontologydesignpatterns.org/ont/dul/DUL.owl#isMemberOf"/>
    


    <!-- http://www.ontologydesignpatterns.org/ont/dul/DUL.owl#isParameterFor -->

    <owl:ObjectProperty rdf:about="http://www.ontologydesignpatterns.org/ont/dul/DUL.owl#isParameterFor">
        <rdfs:subPropertyOf rdf:resource="http://www.ontologydesignpatterns.org/ont/dul/DUL.owl#isRelatedToConcept"/>
        <rdfs:domain rdf:resource="http://www.ontologydesignpatterns.org/ont/dul/DUL.owl#Parameter"/>
        <rdfs:range rdf:resource="http://www.ontologydesignpatterns.org/ont/dul/DUL.owl#Concept"/>
        <rdfs:comment>A Concept can have a Parameter that constrains the attributes that a classified Entity can have in a certain Situation, e.g. a 4WheelDriver Role definedIn the ItalianTrafficLaw has a MinimumAge parameter on the Amount 16.</rdfs:comment>
        <rdfs:isDefinedBy rdf:resource="http://www.ontologydesignpatterns.org/ont/dul/DUL.owl"/>
        <rdfs:label xml:lang="en">is parameter for</rdfs:label>
        <rdfs:label xml:lang="it">è un parametro per</rdfs:label>
    </owl:ObjectProperty>
    


    <!-- http://www.ontologydesignpatterns.org/ont/dul/DUL.owl#isParametrizedBy -->

    <owl:ObjectProperty rdf:about="http://www.ontologydesignpatterns.org/ont/dul/DUL.owl#isParametrizedBy">
        <rdfs:range rdf:resource="http://www.ontologydesignpatterns.org/ont/dul/DUL.owl#Parameter"/>
    </owl:ObjectProperty>
    


    <!-- http://www.ontologydesignpatterns.org/ont/dul/DUL.owl#isRelatedToConcept -->

    <owl:ObjectProperty rdf:about="http://www.ontologydesignpatterns.org/ont/dul/DUL.owl#isRelatedToConcept">
        <rdfs:subPropertyOf rdf:resource="http://www.ontologydesignpatterns.org/ont/dul/DUL.owl#associatedWith"/>
        <owl:inverseOf rdf:resource="http://www.ontologydesignpatterns.org/ont/dul/DUL.owl#isRelatedToConcept"/>
        <rdf:type rdf:resource="http://www.w3.org/2002/07/owl#SymmetricProperty"/>
        <rdfs:domain rdf:resource="http://www.ontologydesignpatterns.org/ont/dul/DUL.owl#Concept"/>
        <rdfs:range rdf:resource="http://www.ontologydesignpatterns.org/ont/dul/DUL.owl#Concept"/>
        <rdfs:comment>Any relation between concepts, e.g. superordinated, conceptual parthood, having a parameter, having a task, superordination, etc.</rdfs:comment>
        <rdfs:isDefinedBy rdf:resource="http://www.ontologydesignpatterns.org/ont/dul/DUL.owl"/>
        <rdfs:label xml:lang="en">is related to concept</rdfs:label>
        <rdfs:label xml:lang="it">è associato al concetto</rdfs:label>
    </owl:ObjectProperty>
    


    <!-- http://www.ontologydesignpatterns.org/ont/dul/DUL.owl#parametrizes -->

    <owl:ObjectProperty rdf:about="http://www.ontologydesignpatterns.org/ont/dul/DUL.owl#parametrizes">
        <rdfs:domain rdf:resource="http://www.ontologydesignpatterns.org/ont/dul/DUL.owl#Parameter"/>
    </owl:ObjectProperty>
    


    <!-- http://www.w3.org/ns/odrl/2/assignee -->

    <owl:ObjectProperty rdf:about="http://www.w3.org/ns/odrl/2/assignee"/>
    


    <!-- http://www.w3.org/ns/odrl/2/assigner -->

    <owl:ObjectProperty rdf:about="http://www.w3.org/ns/odrl/2/assigner"/>
    


    <!-- http://www.w3.org/ns/odrl/2/constraint -->

    <owl:ObjectProperty rdf:about="http://www.w3.org/ns/odrl/2/constraint"/>
    


    <!-- http://www.w3.org/ns/odrl/2/leftOperand -->

    <owl:ObjectProperty rdf:about="http://www.w3.org/ns/odrl/2/leftOperand"/>
    


    <!-- http://www.w3.org/ns/odrl/2/operator -->

    <owl:ObjectProperty rdf:about="http://www.w3.org/ns/odrl/2/operator"/>
    


    <!-- http://www.w3.org/ns/odrl/2/rightOperand -->

    <owl:ObjectProperty rdf:about="http://www.w3.org/ns/odrl/2/rightOperand"/>
    


    <!-- http://www.w3.org/ns/odrl/2/target -->

    <owl:ObjectProperty rdf:about="http://www.w3.org/ns/odrl/2/target"/>
    


    <!-- https://w3id.org/def/vaeontology#abidesByValue -->

    <owl:ObjectProperty rdf:about="https://w3id.org/def/vaeontology#abidesByValue"/>
    


    <!-- https://w3id.org/def/vaeontology#composedBySequence -->

    <owl:ObjectProperty rdf:about="https://w3id.org/def/vaeontology#composedBySequence"/>
    


    <!-- https://w3id.org/def/vaeontology#hasClaim -->

    <owl:ObjectProperty rdf:about="https://w3id.org/def/vaeontology#hasClaim"/>
    


    <!-- https://w3id.org/def/vaeontology#hasInput -->

    <owl:ObjectProperty rdf:about="https://w3id.org/def/vaeontology#hasInput"/>
    


    <!-- https://w3id.org/def/vaeontology#hasOutcome -->

    <owl:ObjectProperty rdf:about="https://w3id.org/def/vaeontology#hasOutcome"/>
    


    <!-- https://w3id.org/def/vaeontology#hasPremise -->

    <owl:ObjectProperty rdf:about="https://w3id.org/def/vaeontology#hasPremise"/>
    


    <!-- https://w3id.org/def/vaeontology#hasState -->

    <owl:ObjectProperty rdf:about="https://w3id.org/def/vaeontology#hasState"/>
    


    <!-- https://w3id.org/def/vaeontology#influencesOutcome -->

    <owl:ObjectProperty rdf:about="https://w3id.org/def/vaeontology#influencesOutcome"/>
    


    <!-- https://w3id.org/def/vaeontology#interpretationOn -->

    <owl:ObjectProperty rdf:about="https://w3id.org/def/vaeontology#interpretationOn"/>
    


    <!-- https://w3id.org/def/vaeontology#isAgentOfSystem -->

    <owl:ObjectProperty rdf:about="https://w3id.org/def/vaeontology#isAgentOfSystem"/>
    


    <!-- https://w3id.org/def/vaeontology#isBasedOnCriterion -->

    <owl:ObjectProperty rdf:about="https://w3id.org/def/vaeontology#isBasedOnCriterion"/>
    


    <!-- https://w3id.org/def/vaeontology#isInputOf -->

    <owl:ObjectProperty rdf:about="https://w3id.org/def/vaeontology#isInputOf"/>
    


    <!-- https://w3id.org/def/vaeontology#isInputOutcomeOf -->

    <owl:ObjectProperty rdf:about="https://w3id.org/def/vaeontology#isInputOutcomeOf"/>
    


    <!-- https://w3id.org/def/vaeontology#isOptimizationOfProperty -->

    <owl:ObjectProperty rdf:about="https://w3id.org/def/vaeontology#isOptimizationOfProperty"/>
    


    <!-- https://w3id.org/def/vaeontology#isOutcomeOf -->

    <owl:ObjectProperty rdf:about="https://w3id.org/def/vaeontology#isOutcomeOf"/>
    


    <!-- https://w3id.org/def/vaeontology#isStartOfSequence -->

    <owl:ObjectProperty rdf:about="https://w3id.org/def/vaeontology#isStartOfSequence"/>
    


    <!-- https://w3id.org/def/vaeontology#isStateOfAgent -->

    <owl:ObjectProperty rdf:about="https://w3id.org/def/vaeontology#isStateOfAgent"/>
    


    <!-- https://w3id.org/def/vaeontology#madeByAgent -->

    <owl:ObjectProperty rdf:about="https://w3id.org/def/vaeontology#madeByAgent"/>
    


    <!-- https://w3id.org/def/vaeontology#makesAction -->

    <owl:ObjectProperty rdf:about="https://w3id.org/def/vaeontology#makesAction"/>
    


    <!-- https://w3id.org/def/vaeontology#measuredOnConditionedEntity -->

    <owl:ObjectProperty rdf:about="https://w3id.org/def/vaeontology#measuredOnConditionedEntity"/>
    


    <!-- https://w3id.org/def/vaeontology#nextInputOutcome -->

    <owl:ObjectProperty rdf:about="https://w3id.org/def/vaeontology#nextInputOutcome"/>
    


    <!-- https://w3id.org/def/vaeontology#onEntity -->

    <owl:ObjectProperty rdf:about="https://w3id.org/def/vaeontology#onEntity"/>
    


    <!-- https://w3id.org/def/vaeontology#propertyExpressedAt -->

    <owl:ObjectProperty rdf:about="https://w3id.org/def/vaeontology#propertyExpressedAt"/>
    


    <!-- https://w3id.org/def/vaeontology#propertyOptimizedAt -->

    <owl:ObjectProperty rdf:about="https://w3id.org/def/vaeontology#propertyOptimizedAt"/>
    


    <!-- https://w3id.org/def/vaeontology#proposesStatement -->

    <owl:ObjectProperty rdf:about="https://w3id.org/def/vaeontology#proposesStatement"/>
    


    <!-- https://w3id.org/def/vaeontology#reflectsValue -->

    <owl:ObjectProperty rdf:about="https://w3id.org/def/vaeontology#reflectsValue"/>
    


    <!-- https://w3id.org/def/vaeontology#relationWith -->

    <owl:ObjectProperty rdf:about="https://w3id.org/def/vaeontology#relationWith"/>
    


    <!-- https://w3id.org/def/vaeontology#satisfiesNorm -->

    <owl:ObjectProperty rdf:about="https://w3id.org/def/vaeontology#satisfiesNorm"/>
    


    <!-- https://w3id.org/def/vaeontology#startsWithInputOutcome -->

    <owl:ObjectProperty rdf:about="https://w3id.org/def/vaeontology#startsWithInputOutcome"/>
    


    <!-- https://w3id.org/def/vaeontology_montes_sierra#hasOutState -->

    <owl:ObjectProperty rdf:about="https://w3id.org/def/vaeontology_montes_sierra#hasOutState">
        <rdfs:subPropertyOf rdf:resource="http://www.ontologydesignpatterns.org/ont/dul/DUL.owl#hasConstituent"/>
        <owl:inverseOf rdf:resource="https://w3id.org/def/vaeontology_montes_sierra#isOutStateOf"/>
        <rdfs:domain rdf:resource="https://w3id.org/def/vaeontology#Path"/>
        <rdfs:range rdf:resource="https://w3id.org/def/vaeontology#State"/>
        <rdfs:comment>&quot;Given a path p ∈ P, the function out : P → S returns the last state (or the outcome) of path p, out(p) = sn.&quot;</rdfs:comment>
        <rdfs:label>hasOutState</rdfs:label>
        <bhv:bibRef>Montes, N., Sierra, C.: Synthesis and properties of optimally value-aligned nor-
mative systems. Journal of Artificial Intelligence Research 74, 1739–1774 (2022).
https://doi.org/10.1613/jair.1.13487</bhv:bibRef>
    </owl:ObjectProperty>
    


    <!-- https://w3id.org/def/vaeontology_montes_sierra#isOutStateOf -->

    <owl:ObjectProperty rdf:about="https://w3id.org/def/vaeontology_montes_sierra#isOutStateOf">
        <rdfs:subPropertyOf rdf:resource="http://www.ontologydesignpatterns.org/ont/dul/DUL.owl#isConstituentOf"/>
        <rdfs:domain rdf:resource="https://w3id.org/def/vaeontology#State"/>
        <rdfs:range rdf:resource="https://w3id.org/def/vaeontology#Path"/>
        <rdfs:comment>&quot;Given a path p ∈ P, the function out : P → S returns the last state (or the outcome) of path p, out(p) = sn.&quot;</rdfs:comment>
        <rdfs:label>isOutStateOf</rdfs:label>
        <bhv:bibRef>Montes, N., Sierra, C.: Synthesis and properties of optimally value-aligned nor-
mative systems. Journal of Artificial Intelligence Research 74, 1739–1774 (2022).
https://doi.org/10.1613/jair.1.13487</bhv:bibRef>
    </owl:ObjectProperty>
    


    <!-- 
    ///////////////////////////////////////////////////////////////////////////////////////
    //
    // Data properties
    //
    ///////////////////////////////////////////////////////////////////////////////////////
     -->

    


    <!-- http://www.ontologydesignpatterns.org/ont/dul/DUL.owl#hasDataValue -->

    <owl:DatatypeProperty rdf:about="http://www.ontologydesignpatterns.org/ont/dul/DUL.owl#hasDataValue"/>
    


    <!-- http://www.ontologydesignpatterns.org/ont/dul/DUL.owl#hasParameterDataValue -->

    <owl:DatatypeProperty rdf:about="http://www.ontologydesignpatterns.org/ont/dul/DUL.owl#hasParameterDataValue">
        <rdfs:subPropertyOf rdf:resource="http://www.ontologydesignpatterns.org/ont/dul/DUL.owl#hasDataValue"/>
        <rdfs:domain rdf:resource="http://www.ontologydesignpatterns.org/ont/dul/DUL.owl#Parameter"/>
        <rdfs:comment>Parametrizes values from a datatype. For example, a Parameter MinimumAgeForDriving hasParameterDataValue 18 on datatype xsd:int, in the Italian traffic code. In this example, MinimumAgeForDriving isDefinedIn the Norm ItalianTrafficCodeAgeDriving.
More complex parametrization requires workarounds. E.g. AgeRangeForDrugUsage could parametrize data value: 14 to 50 on the datatype: xsd:int. Since complex datatypes are not allowed in OWL1.0, a solution to this can only work by creating two &apos;sub-parameters&apos;: MinimumAgeForDrugUsage (that hasParameterDataValue 14) and MaximumAgeForDrugUsage (that hasParameterDataValue 50), which are components of (cf. hasComponent) the main Parameter AgeRangeForDrugUsage.
Ordering on subparameters can be created by using or specializing the object property &apos;precedes&apos;.</rdfs:comment>
        <rdfs:isDefinedBy rdf:resource="http://www.ontologydesignpatterns.org/ont/dul/DUL.owl"/>
        <rdfs:label xml:lang="it">ha valore</rdfs:label>
        <rdfs:label xml:lang="en">has parameter data value</rdfs:label>
    </owl:DatatypeProperty>
    


    <!-- http://www.w3.org/1999/02/22-rdf-syntax-ns#value -->

    <owl:DatatypeProperty rdf:about="http://www.w3.org/1999/02/22-rdf-syntax-ns#value"/>
    


    <!-- https://w3id.org/def/vaeontology_montes_sierra#belongsToSegment -->

    <owl:DatatypeProperty rdf:about="https://w3id.org/def/vaeontology_montes_sierra#belongsToSegment">
        <rdfs:subPropertyOf rdf:resource="http://www.ontologydesignpatterns.org/ont/dul/DUL.owl#hasDataValue"/>
        <rdf:type rdf:resource="http://www.w3.org/2002/07/owl#FunctionalProperty"/>
        <rdfs:domain rdf:resource="https://w3id.org/def/vaeontology_montes_sierra#TaxingAgentState"/>
        <rdfs:range>
            <rdfs:Datatype>
                <owl:oneOf>
                    <rdf:Description>
                        <rdf:type rdf:resource="http://www.w3.org/1999/02/22-rdf-syntax-ns#List"/>
                        <rdf:first rdf:datatype="http://www.w3.org/2001/XMLSchema#integer">1</rdf:first>
                        <rdf:rest>
                            <rdf:Description>
                                <rdf:type rdf:resource="http://www.w3.org/1999/02/22-rdf-syntax-ns#List"/>
                                <rdf:first rdf:datatype="http://www.w3.org/2001/XMLSchema#integer">2</rdf:first>
                                <rdf:rest>
                                    <rdf:Description>
                                        <rdf:type rdf:resource="http://www.w3.org/1999/02/22-rdf-syntax-ns#List"/>
                                        <rdf:first rdf:datatype="http://www.w3.org/2001/XMLSchema#integer">3</rdf:first>
                                        <rdf:rest>
                                            <rdf:Description>
                                                <rdf:type rdf:resource="http://www.w3.org/1999/02/22-rdf-syntax-ns#List"/>
                                                <rdf:first rdf:datatype="http://www.w3.org/2001/XMLSchema#integer">4</rdf:first>
                                                <rdf:rest>
                                                    <rdf:Description>
                                                        <rdf:type rdf:resource="http://www.w3.org/1999/02/22-rdf-syntax-ns#List"/>
                                                        <rdf:first rdf:datatype="http://www.w3.org/2001/XMLSchema#integer">5</rdf:first>
                                                        <rdf:rest rdf:resource="http://www.w3.org/1999/02/22-rdf-syntax-ns#nil"/>
                                                    </rdf:Description>
                                                </rdf:rest>
                                            </rdf:Description>
                                        </rdf:rest>
                                    </rdf:Description>
                                </rdf:rest>
                            </rdf:Description>
                        </rdf:rest>
                    </rdf:Description>
                </owl:oneOf>
            </rdfs:Datatype>
        </rdfs:range>
        <rdfs:comment>&quot;At any given time-step, every agent is characterised by its current wealth xi as well as an integer that denotes the wealth segment it belongs to.&quot;</rdfs:comment>
        <rdfs:label>belongsToSegment</rdfs:label>
    </owl:DatatypeProperty>
    


    <!-- https://w3id.org/def/vaeontology_montes_sierra#hasProbabilityOrFraction -->

    <owl:DatatypeProperty rdf:about="https://w3id.org/def/vaeontology_montes_sierra#hasProbabilityOrFraction">
        <rdfs:subPropertyOf rdf:resource="http://www.ontologydesignpatterns.org/ont/dul/DUL.owl#hasParameterDataValue"/>
        <rdf:type rdf:resource="http://www.w3.org/2002/07/owl#FunctionalProperty"/>
        <rdfs:domain rdf:resource="http://www.ontologydesignpatterns.org/ont/dul/DUL.owl#Parameter"/>
        <rdfs:range>
            <rdfs:Datatype>
                <owl:onDatatype rdf:resource="http://www.w3.org/2001/XMLSchema#decimal"/>
                <owl:withRestrictions rdf:parseType="Collection">
                    <rdf:Description>
                        <xsd:minInclusive rdf:datatype="http://www.w3.org/2001/XMLSchema#decimal">0.0</xsd:minInclusive>
                    </rdf:Description>
                    <rdf:Description>
                        <xsd:maxInclusive rdf:datatype="http://www.w3.org/2001/XMLSchema#decimal">1.0</xsd:maxInclusive>
                    </rdf:Description>
                </owl:withRestrictions>
            </rdfs:Datatype>
        </rdfs:range>
        <rdfs:comment>Reference to a probability or fraction, e.g. the probability of catching an evader, or the fraction of the fund to be redistributed back to a segment.</rdfs:comment>
        <rdfs:label>hasProbabilityOrFraction</rdfs:label>
    </owl:DatatypeProperty>
    


    <!-- https://w3id.org/def/vaeontology_montes_sierra#hasWealth -->

    <owl:DatatypeProperty rdf:about="https://w3id.org/def/vaeontology_montes_sierra#hasWealth">
        <rdfs:subPropertyOf rdf:resource="http://www.ontologydesignpatterns.org/ont/dul/DUL.owl#hasDataValue"/>
        <rdf:type rdf:resource="http://www.w3.org/2002/07/owl#FunctionalProperty"/>
        <rdfs:domain rdf:resource="https://w3id.org/def/vaeontology_montes_sierra#TaxingAgentState"/>
        <rdfs:range rdf:resource="http://www.w3.org/2001/XMLSchema#decimal"/>
        <rdfs:comment>&quot;At any given time-step, every agent is characterised by its current wealth xi as well as an integer that denotes the wealth segment it belongs to.&quot;</rdfs:comment>
        <rdfs:label>hasWealth</rdfs:label>
    </owl:DatatypeProperty>
    


    <!-- 
    ///////////////////////////////////////////////////////////////////////////////////////
    //
    // Classes
    //
    ///////////////////////////////////////////////////////////////////////////////////////
     -->

    


    <!-- http://www.ontologydesignpatterns.org/ont/dul/DUL.owl#Collection -->

    <owl:Class rdf:about="http://www.ontologydesignpatterns.org/ont/dul/DUL.owl#Collection"/>
    


    <!-- http://www.ontologydesignpatterns.org/ont/dul/DUL.owl#Concept -->

    <owl:Class rdf:about="http://www.ontologydesignpatterns.org/ont/dul/DUL.owl#Concept">
        <rdfs:subClassOf rdf:resource="http://www.ontologydesignpatterns.org/ont/dul/DUL.owl#SocialObject"/>
    </owl:Class>
    


    <!-- http://www.ontologydesignpatterns.org/ont/dul/DUL.owl#EventType -->

    <owl:Class rdf:about="http://www.ontologydesignpatterns.org/ont/dul/DUL.owl#EventType">
        <owl:disjointWith rdf:resource="http://www.ontologydesignpatterns.org/ont/dul/DUL.owl#Parameter"/>
    </owl:Class>
    


    <!-- http://www.ontologydesignpatterns.org/ont/dul/DUL.owl#Parameter -->

    <owl:Class rdf:about="http://www.ontologydesignpatterns.org/ont/dul/DUL.owl#Parameter">
        <rdfs:subClassOf rdf:resource="http://www.ontologydesignpatterns.org/ont/dul/DUL.owl#Concept"/>
        <rdfs:subClassOf>
            <owl:Restriction>
                <owl:onProperty rdf:resource="http://www.ontologydesignpatterns.org/ont/dul/DUL.owl#classifies"/>
                <owl:allValuesFrom rdf:resource="http://www.ontologydesignpatterns.org/ont/dul/DUL.owl#Region"/>
            </owl:Restriction>
        </rdfs:subClassOf>
        <rdfs:subClassOf>
            <owl:Restriction>
                <owl:onProperty rdf:resource="http://www.ontologydesignpatterns.org/ont/dul/DUL.owl#hasPart"/>
                <owl:allValuesFrom rdf:resource="http://www.ontologydesignpatterns.org/ont/dul/DUL.owl#Parameter"/>
            </owl:Restriction>
        </rdfs:subClassOf>
        <owl:disjointWith rdf:resource="http://www.ontologydesignpatterns.org/ont/dul/DUL.owl#Role"/>
        <rdfs:comment>A Concept that classifies a Region; the difference between a Region and a Parameter is that regions represent sets of observable values, e.g. the height  of a given building, while parameters represent constraints or selections on observable values, e.g. &apos;VeryHigh&apos;. Therefore, parameters can also be used to constrain regions, e.g. VeryHigh on a subset of values of the Region Height applied to buildings, or to add an external selection criterion , such as measurement units, to regions, e.g. Meter on a subset of values from the Region Length applied to the Region Length applied to roads.</rdfs:comment>
        <rdfs:isDefinedBy rdf:resource="http://www.ontologydesignpatterns.org/ont/dul/DUL.owl"/>
        <rdfs:label xml:lang="en">Parameter</rdfs:label>
        <rdfs:label xml:lang="it">Parametro</rdfs:label>
    </owl:Class>
    


    <!-- http://www.ontologydesignpatterns.org/ont/dul/DUL.owl#Region -->

    <owl:Class rdf:about="http://www.ontologydesignpatterns.org/ont/dul/DUL.owl#Region"/>
    


    <!-- http://www.ontologydesignpatterns.org/ont/dul/DUL.owl#Role -->

    <owl:Class rdf:about="http://www.ontologydesignpatterns.org/ont/dul/DUL.owl#Role"/>
    


    <!-- http://www.ontologydesignpatterns.org/ont/dul/DUL.owl#SocialObject -->

    <owl:Class rdf:about="http://www.ontologydesignpatterns.org/ont/dul/DUL.owl#SocialObject"/>
    


    <!-- http://www.ontologydesignpatterns.org/ont/dul/DUL.owl#UnitOfMeasure -->

    <owl:Class rdf:about="http://www.ontologydesignpatterns.org/ont/dul/DUL.owl#UnitOfMeasure">
        <rdfs:subClassOf rdf:resource="http://www.ontologydesignpatterns.org/ont/dul/DUL.owl#Parameter"/>
    </owl:Class>
    


    <!-- http://www.w3.org/ns/odrl/2/Constraint -->

    <owl:Class rdf:about="http://www.w3.org/ns/odrl/2/Constraint"/>
    


    <!-- https://w3id.org/def/vaeontology#ActingAgent -->

    <owl:Class rdf:about="https://w3id.org/def/vaeontology#ActingAgent"/>
    


    <!-- https://w3id.org/def/vaeontology#Action -->

    <owl:Class rdf:about="https://w3id.org/def/vaeontology#Action"/>
    


    <!-- https://w3id.org/def/vaeontology#AggregationFunction -->

    <owl:Class rdf:about="https://w3id.org/def/vaeontology#AggregationFunction"/>
    


    <!-- https://w3id.org/def/vaeontology#AlignmentStatement -->

    <owl:Class rdf:about="https://w3id.org/def/vaeontology#AlignmentStatement"/>
    


    <!-- https://w3id.org/def/vaeontology#ArgumentStatement -->

    <owl:Class rdf:about="https://w3id.org/def/vaeontology#ArgumentStatement"/>
    


    <!-- https://w3id.org/def/vaeontology#Context -->

    <owl:Class rdf:about="https://w3id.org/def/vaeontology#Context"/>
    


    <!-- https://w3id.org/def/vaeontology#Criterion -->

    <owl:Class rdf:about="https://w3id.org/def/vaeontology#Criterion"/>
    


    <!-- https://w3id.org/def/vaeontology#Equality -->

    <owl:Class rdf:about="https://w3id.org/def/vaeontology#Equality">
        <rdfs:comment>&quot;First, we ground the meaning of value equality in the context of our model as, of course, economic equality.&quot;</rdfs:comment>
    </owl:Class>
    


    <!-- https://w3id.org/def/vaeontology#FinalInputOutcome -->

    <owl:Class rdf:about="https://w3id.org/def/vaeontology#FinalInputOutcome"/>
    


    <!-- https://w3id.org/def/vaeontology#MultiInputOutcome -->

    <owl:Class rdf:about="https://w3id.org/def/vaeontology#MultiInputOutcome"/>
    


    <!-- https://w3id.org/def/vaeontology#Norm -->

    <owl:Class rdf:about="https://w3id.org/def/vaeontology#Norm"/>
    


    <!-- https://w3id.org/def/vaeontology#OptimizedProperty -->

    <owl:Class rdf:about="https://w3id.org/def/vaeontology#OptimizedProperty"/>
    


    <!-- https://w3id.org/def/vaeontology#Path -->

    <owl:Class rdf:about="https://w3id.org/def/vaeontology#Path">
        <rdfs:subClassOf>
            <owl:Restriction>
                <owl:onProperty rdf:resource="https://w3id.org/def/vaeontology_montes_sierra#hasOutState"/>
                <owl:someValuesFrom>
                    <owl:Class>
                        <owl:intersectionOf rdf:parseType="Collection">
                            <rdf:Description rdf:about="https://w3id.org/def/vaeontology#State"/>
                            <owl:Restriction>
                                <owl:onProperty rdf:resource="https://w3id.org/def/vaeontology#isOutcomeOf"/>
                                <owl:someValuesFrom rdf:resource="https://w3id.org/def/vaeontology#FinalInputOutcome"/>
                            </owl:Restriction>
                        </owl:intersectionOf>
                    </owl:Class>
                </owl:someValuesFrom>
            </owl:Restriction>
        </rdfs:subClassOf>
    </owl:Class>
    


    <!-- https://w3id.org/def/vaeontology#QuantitativePromotionDemotion -->

    <owl:Class rdf:about="https://w3id.org/def/vaeontology#QuantitativePromotionDemotion"/>
    


    <!-- https://w3id.org/def/vaeontology#QuantitativeVaeProperty -->

    <owl:Class rdf:about="https://w3id.org/def/vaeontology#QuantitativeVaeProperty"/>
    


    <!-- https://w3id.org/def/vaeontology#Sequence -->

    <owl:Class rdf:about="https://w3id.org/def/vaeontology#Sequence"/>
    


    <!-- https://w3id.org/def/vaeontology#State -->

    <owl:Class rdf:about="https://w3id.org/def/vaeontology#State"/>
    


    <!-- https://w3id.org/def/vaeontology#System -->

    <owl:Class rdf:about="https://w3id.org/def/vaeontology#System"/>
    


    <!-- https://w3id.org/def/vaeontology#Transition -->

    <owl:Class rdf:about="https://w3id.org/def/vaeontology#Transition"/>
    


    <!-- https://w3id.org/def/vaeontology#User -->

    <owl:Class rdf:about="https://w3id.org/def/vaeontology#User"/>
    


    <!-- https://w3id.org/def/vaeontology#ValueProperty -->

    <owl:Class rdf:about="https://w3id.org/def/vaeontology#ValueProperty"/>
    


    <!-- https://w3id.org/def/vaeontology_montes_sierra#BoundedQuantitativePromotionDemotion -->

    <owl:Class rdf:about="https://w3id.org/def/vaeontology_montes_sierra#BoundedQuantitativePromotionDemotion">
        <rdfs:subClassOf rdf:resource="https://w3id.org/def/vaeontology#QuantitativePromotionDemotion"/>
        <rdfs:subClassOf>
            <owl:Restriction>
                <owl:onProperty rdf:resource="http://www.w3.org/1999/02/22-rdf-syntax-ns#value"/>
                <owl:allValuesFrom>
                    <rdfs:Datatype>
                        <owl:onDatatype rdf:resource="http://www.w3.org/2002/07/owl#real"/>
                        <owl:withRestrictions rdf:parseType="Collection">
                            <rdf:Description>
                                <xsd:minInclusive rdf:datatype="http://www.w3.org/2001/XMLSchema#decimal">-1.0</xsd:minInclusive>
                            </rdf:Description>
                            <rdf:Description>
                                <xsd:maxInclusive rdf:datatype="http://www.w3.org/2001/XMLSchema#decimal">1.0</xsd:maxInclusive>
                            </rdf:Description>
                        </owl:withRestrictions>
                    </rdfs:Datatype>
                </owl:allValuesFrom>
            </owl:Restriction>
        </rdfs:subClassOf>
        <rdfs:label>BoundedQuantitativePromotionDemotion</rdfs:label>
        <skos:definition>A quantitative Promotion or Demotion, bounded in a certain interval where the limits -1 and 1 represent the highest degrees of promotion and demotion, and the centre (0) the neutrality.</skos:definition>
    </owl:Class>
    


    <!-- https://w3id.org/def/vaeontology_montes_sierra#EvaderAgent -->

    <owl:Class rdf:about="https://w3id.org/def/vaeontology_montes_sierra#EvaderAgent">
        <rdfs:subClassOf rdf:resource="https://w3id.org/def/vaeontology_montes_sierra#TaxingAgent"/>
        <rdfs:subClassOf>
            <owl:Restriction>
                <owl:onProperty rdf:resource="https://w3id.org/def/vaeontology#makesAction"/>
                <owl:allValuesFrom rdf:resource="https://w3id.org/def/vaeontology_montes_sierra#NotPayingTaxesTransaction"/>
            </owl:Restriction>
        </rdfs:subClassOf>
        <rdfs:comment>&quot;In our running example, the MAS is composed of a set of 200 agents G = {1, 2, ..., 200}. Of these 200, we set 10 to be “evader” agents, which will try to skip payment when the tax collection and redistribution scheme is imposed. This composition of the society (10 out of 200 evader agents) is an arbitrary choice made for exemplification purposes.&quot;</rdfs:comment>
        <rdfs:label>EvaderAgent</rdfs:label>
    </owl:Class>
    


    <!-- https://w3id.org/def/vaeontology_montes_sierra#Fairness -->

    <owl:Class rdf:about="https://w3id.org/def/vaeontology_montes_sierra#Fairness">
        <rdfs:subClassOf rdf:resource="https://w3id.org/spice/SON/SchwartzValues#SelfTrascendence"/>
        <rdfs:comment>&quot;Second, we ground the semantics of value fairness to mean that evader individuals should be punished for their evasion.&quot;</rdfs:comment>
        <rdfs:label>Fairness</rdfs:label>
    </owl:Class>
    


    <!-- https://w3id.org/def/vaeontology_montes_sierra#GiniIndex -->

    <owl:Class rdf:about="https://w3id.org/def/vaeontology_montes_sierra#GiniIndex">
        <rdfs:subClassOf rdf:resource="https://w3id.org/def/vaeontology_montes_sierra#SemanticsFunction"/>
        <rdfs:subClassOf>
            <owl:Restriction>
                <owl:onProperty rdf:resource="https://w3id.org/def/vaeontology#relationWith"/>
                <owl:allValuesFrom rdf:resource="https://w3id.org/def/vaeontology#Equality"/>
            </owl:Restriction>
        </rdfs:subClassOf>
        <rdfs:comment>&quot;First, we ground the meaning of value equality in the context of our model as, of course, economic equality. To do so, we use the well-known Gini index indicator (Gini, 1912), a widespread metric to quantify wealth and income inequality (The World Bank, Development Research Group, 2019).&quot;</rdfs:comment>
        <rdfs:comment>The Gini Index can be used as a Semantics Function in State, as in the taxing problem from Montes and Sierra (see reference).</rdfs:comment>
        <rdfs:label>Gini Index</rdfs:label>
        <bhv:bibRef>Montes, N., Sierra, C.: Synthesis and properties of optimally value-aligned nor-
mative systems. Journal of Artificial Intelligence Research 74, 1739–1774 (2022).
https://doi.org/10.1613/jair.1.13487</bhv:bibRef>
    </owl:Class>
    


    <!-- https://w3id.org/def/vaeontology_montes_sierra#LegalAgent -->

    <owl:Class rdf:about="https://w3id.org/def/vaeontology_montes_sierra#LegalAgent">
        <rdfs:subClassOf rdf:resource="https://w3id.org/def/vaeontology_montes_sierra#TaxingAgent"/>
        <rdfs:subClassOf>
            <owl:Restriction>
                <owl:onProperty rdf:resource="https://w3id.org/def/vaeontology#makesAction"/>
                <owl:allValuesFrom rdf:resource="https://w3id.org/def/vaeontology_montes_sierra#PayingTaxesTransaction"/>
            </owl:Restriction>
        </rdfs:subClassOf>
        <rdfs:comment>&quot;In our running example, the MAS is composed of a set of 200 agents G = {1, 2, ..., 200}. Of these 200, we set 10 to be “evader” agents, which will try to skip payment when the tax collection and redistribution scheme is imposed. This composition of the society (10 out of 200 evader agents) is an arbitrary choice made for exemplification purposes.&quot;</rdfs:comment>
        <rdfs:label>LegalAgent</rdfs:label>
    </owl:Class>
    


    <!-- https://w3id.org/def/vaeontology_montes_sierra#MoneyTransaction -->

    <owl:Class rdf:about="https://w3id.org/def/vaeontology_montes_sierra#MoneyTransaction">
        <rdfs:subClassOf rdf:resource="https://w3id.org/def/vaeontology#Action"/>
        <rdfs:comment>&quot;In principle, in the unregulated situation agents can exchange money as they see fit at any transition.&quot;</rdfs:comment>
        <rdfs:label>MoneyTransaction</rdfs:label>
        <skos:definition>Any kind of action made by agents in the TaxingSystem.</skos:definition>
    </owl:Class>
    


    <!-- https://w3id.org/def/vaeontology_montes_sierra#NormativeSystem -->

    <owl:Class rdf:about="https://w3id.org/def/vaeontology_montes_sierra#NormativeSystem">
        <rdfs:subClassOf rdf:resource="http://www.ontologydesignpatterns.org/ont/dul/DUL.owl#Collection"/>
        <rdfs:subClassOf rdf:resource="https://w3id.org/def/vaeontology#Norm"/>
        <rdfs:subClassOf>
            <owl:Restriction>
                <owl:onProperty rdf:resource="http://www.ontologydesignpatterns.org/ont/dul/DUL.owl#hasConstituent"/>
                <owl:someValuesFrom rdf:resource="https://w3id.org/def/vaeontology_montes_sierra#ParametricNorm"/>
            </owl:Restriction>
        </rdfs:subClassOf>
        <rdfs:comment>&quot;A normative system N is a set of individual norms {ni} with all of their parameters instantiated to some quantity&quot;</rdfs:comment>
        <rdfs:label>NormativeSystem</rdfs:label>
    </owl:Class>
    


    <!-- https://w3id.org/def/vaeontology_montes_sierra#NormativeSystemAlignment -->

    <owl:Class rdf:about="https://w3id.org/def/vaeontology_montes_sierra#NormativeSystemAlignment">
        <rdfs:subClassOf rdf:resource="https://w3id.org/def/vaeontology#ValueProperty"/>
        <rdfs:subClassOf rdf:resource="https://w3id.org/def/vaeontology_montes_sierra#BoundedQuantitativePromotionDemotion"/>
        <rdfs:subClassOf>
            <owl:Restriction>
                <owl:onProperty rdf:resource="https://w3id.org/def/vaeontology#propertyExpressedAt"/>
                <owl:someValuesFrom>
                    <owl:Class>
                        <owl:intersectionOf rdf:parseType="Collection">
                            <rdf:Description rdf:about="https://w3id.org/def/vaeontology#AlignmentStatement"/>
                            <owl:Restriction>
                                <owl:onProperty rdf:resource="https://w3id.org/def/vaeontology#onEntity"/>
                                <owl:someValuesFrom rdf:resource="https://w3id.org/def/vaeontology_montes_sierra#NormativeSystem"/>
                            </owl:Restriction>
                        </owl:intersectionOf>
                    </owl:Class>
                </owl:someValuesFrom>
            </owl:Restriction>
        </rdfs:subClassOf>
        <rdfs:subClassOf>
            <owl:Restriction>
                <owl:onProperty rdf:resource="https://w3id.org/def/vaeontology#measuredOnConditionedEntity"/>
                <owl:allValuesFrom>
                    <owl:Class>
                        <owl:intersectionOf rdf:parseType="Collection">
                            <owl:Class>
                                <owl:unionOf rdf:parseType="Collection">
                                    <rdf:Description rdf:about="https://w3id.org/def/vaeontology#Path"/>
                                    <owl:Class>
                                        <owl:intersectionOf rdf:parseType="Collection">
                                            <rdf:Description rdf:about="https://w3id.org/def/vaeontology#State"/>
                                            <owl:Restriction>
                                                <owl:onProperty rdf:resource="https://w3id.org/def/vaeontology_montes_sierra#isOutStateOf"/>
                                                <owl:someValuesFrom rdf:resource="https://w3id.org/def/vaeontology#Path"/>
                                            </owl:Restriction>
                                        </owl:intersectionOf>
                                    </owl:Class>
                                </owl:unionOf>
                            </owl:Class>
                            <owl:Restriction>
                                <owl:onProperty rdf:resource="https://w3id.org/def/vaeontology#satisfiesNorm"/>
                                <owl:someValuesFrom rdf:resource="https://w3id.org/def/vaeontology_montes_sierra#NormativeSystem"/>
                            </owl:Restriction>
                        </owl:intersectionOf>
                    </owl:Class>
                </owl:allValuesFrom>
            </owl:Restriction>
        </rdfs:subClassOf>
        <rdfs:comment>&quot;Definition 4. Given a world (S , A, T ), a normative system N that applies to it, and a set of values V = {v1, ..., vn} with semantics functions f1, ..., fn, the alignment AlgnN,v of normative system N with respect to value v ∈ V is computed as:
(expectancy of the evaluation of a semantics function on the final state of PN) (3)
where PN is the random variable of the subset of paths restricted under the normative system N.&quot;</rdfs:comment>
        <rdfs:comment>Not only about the final state of a path, but can be calculated by another property on the variable PN: &quot;In line with the consequentialist view we present in Section 3, the alignment in eq. (3) is computed by considering the ultimate consequences (i.e. the end-state) that the implementation of a set of norms brings about. However, other alternatives are possible. For example, one may prefer to compute the alignment by considering the value semantics function applied to all the states that are visited during a path. In that case, one would also need to specify how to aggregate the evaluation of fv over all the visited states (e.g. average, minimum...).
&quot;</rdfs:comment>
        <rdfs:label>NormativeSystemAlignment</rdfs:label>
    </owl:Class>
    


    <!-- https://w3id.org/def/vaeontology_montes_sierra#NotPayingTaxesTransaction -->

    <owl:Class rdf:about="https://w3id.org/def/vaeontology_montes_sierra#NotPayingTaxesTransaction">
        <rdfs:subClassOf rdf:resource="https://w3id.org/def/vaeontology_montes_sierra#MoneyTransaction"/>
        <owl:disjointWith rdf:resource="https://w3id.org/def/vaeontology_montes_sierra#PayingTaxesTransaction"/>
        <rdfs:comment>&quot;Agents contribute to the common fund with a tax amount that is dependent on their economic status. However, a subset of evader agents try to skip the payment.&quot;</rdfs:comment>
        <rdfs:label>NotPayingTaxesTransaction</rdfs:label>
        <skos:definition>An action for an agent that does not pay its taxes in the TaxingSystem.</skos:definition>
    </owl:Class>
    


    <!-- https://w3id.org/def/vaeontology_montes_sierra#OptimalNormativeSystemAlignment -->

    <owl:Class rdf:about="https://w3id.org/def/vaeontology_montes_sierra#OptimalNormativeSystemAlignment">
        <rdfs:subClassOf rdf:resource="https://w3id.org/def/vaeontology#OptimizedProperty"/>
        <rdfs:subClassOf rdf:resource="https://w3id.org/def/vaeontology_montes_sierra#NormativeSystemAlignment"/>
        <rdfs:subClassOf>
            <owl:Restriction>
                <owl:onProperty rdf:resource="https://w3id.org/def/vaeontology#propertyOptimizedAt"/>
                <owl:someValuesFrom rdf:resource="https://w3id.org/def/vaeontology_montes_sierra#NormativeSystemAlignment"/>
            </owl:Restriction>
        </rdfs:subClassOf>
        <rdfs:label>OptimalNormativeSystemAlignment</rdfs:label>
    </owl:Class>
    


    <!-- https://w3id.org/def/vaeontology_montes_sierra#ParametricNorm -->

    <owl:Class rdf:about="https://w3id.org/def/vaeontology_montes_sierra#ParametricNorm">
        <rdfs:subClassOf rdf:resource="https://w3id.org/def/vaeontology#Norm"/>
        <rdfs:subClassOf>
            <owl:Restriction>
                <owl:onProperty rdf:resource="http://www.ontologydesignpatterns.org/ont/dul/DUL.owl#isMemberOf"/>
                <owl:someValuesFrom rdf:resource="https://w3id.org/def/vaeontology_montes_sierra#NormativeSystem"/>
            </owl:Restriction>
        </rdfs:subClassOf>
        <rdfs:subClassOf>
            <owl:Restriction>
                <owl:onProperty rdf:resource="http://www.ontologydesignpatterns.org/ont/dul/DUL.owl#hasParameter"/>
                <owl:minQualifiedCardinality rdf:datatype="http://www.w3.org/2001/XMLSchema#nonNegativeInteger">1</owl:minQualifiedCardinality>
                <owl:onClass rdf:resource="http://www.ontologydesignpatterns.org/ont/dul/DUL.owl#Parameter"/>
            </owl:Restriction>
        </rdfs:subClassOf>
        <rdfs:comment>&quot;The main steps of our synthesis approach are: a) [...] b) Define the norms ni in the normative system N that regulate the transitions between consecutive states of the MAS. Every norm targets a particular aspect of the transition. All norms are parametric on a set of values, whose domains and constraints have to be specified. This parametrisation provides the search space N over which the maximising search in eq. (1) is performed.&quot;</rdfs:comment>
        <rdfs:label>ParametricNorm</rdfs:label>
    </owl:Class>
    


    <!-- https://w3id.org/def/vaeontology_montes_sierra#PayingTaxesTransaction -->

    <owl:Class rdf:about="https://w3id.org/def/vaeontology_montes_sierra#PayingTaxesTransaction">
        <rdfs:subClassOf rdf:resource="https://w3id.org/def/vaeontology_montes_sierra#MoneyTransaction"/>
        <rdfs:comment>&quot;Agents contribute to the common fund with a tax amount that is dependent on their economic status.&quot;</rdfs:comment>
        <rdfs:label>PayingTaxesTransaction</rdfs:label>
        <skos:definition>An action for an agent which pays its taxes in the TaxingSystem.</skos:definition>
    </owl:Class>
    


    <!-- https://w3id.org/def/vaeontology_montes_sierra#ProbabilityTaxFairnessSemantics -->

    <owl:Class rdf:about="https://w3id.org/def/vaeontology_montes_sierra#ProbabilityTaxFairnessSemantics">
        <rdfs:subClassOf rdf:resource="https://w3id.org/def/vaeontology_montes_sierra#SemanticsFunction"/>
        <rdfs:comment>&quot;Second, we ground the semantics of value fairness to mean that evader individuals should be punished for their evasion. Hence, we consider that fairness is being highly promoted if, by the end of a fixed-length path, as many evaders as possible belong to the poorest wealth segment</rdfs:comment>
        <rdfs:label>ProbabilityTaxFairnessSemantics</rdfs:label>
    </owl:Class>
    


    <!-- https://w3id.org/def/vaeontology_montes_sierra#SemanticsFunction -->

    <owl:Class rdf:about="https://w3id.org/def/vaeontology_montes_sierra#SemanticsFunction">
        <rdfs:subClassOf rdf:resource="https://w3id.org/def/vaeontology#QuantitativeVaeProperty"/>
        <rdfs:subClassOf rdf:resource="https://w3id.org/def/vaeontology#ValueProperty"/>
        <rdfs:subClassOf rdf:resource="https://w3id.org/def/vaeontology_montes_sierra#BoundedQuantitativePromotionDemotion"/>
        <rdfs:comment>&quot;Given a world (S, A, T ) and a set of values V , the semantics of value v ∈ V in the world is a function fv : S → [−1,1] that evaluates the states of the world, where fv(s) ∼ −1,0,+1 indicates that state s strongly opposes, is neutral or strongly promotes value v, respectively.&quot;</rdfs:comment>
        <rdfs:comment>&quot;To express the relationship between an abstract value and the meaning it takes in a particular context, we say that an explicit goal g grounds the semantics of value v in context C&quot; [Nieves Montes, Carles Sierra et al. https://www.jair.org/index.php/jair/article/view/13487]</rdfs:comment>
        <rdfs:label>Semantics Function</rdfs:label>
        <bhv:bibRef>Montes, N., Sierra, C.: Synthesis and properties of optimally value-aligned nor-
mative systems. Journal of Artificial Intelligence Research 74, 1739–1774 (2022).
https://doi.org/10.1613/jair.1.13487</bhv:bibRef>
    </owl:Class>
    


    <!-- https://w3id.org/def/vaeontology_montes_sierra#SemanticsFunctionAggregation -->

    <owl:Class rdf:about="https://w3id.org/def/vaeontology_montes_sierra#SemanticsFunctionAggregation">
        <rdfs:subClassOf rdf:resource="https://w3id.org/def/vaeontology#AggregationFunction"/>
        <rdfs:subClassOf rdf:resource="https://w3id.org/def/vaeontology_montes_sierra#BoundedQuantitativePromotionDemotion"/>
        <rdfs:subClassOf>
            <owl:Restriction>
                <owl:onProperty rdf:resource="http://www.ontologydesignpatterns.org/ont/dul/DUL.owl#hasConstituent"/>
                <owl:someValuesFrom rdf:resource="https://w3id.org/def/vaeontology_montes_sierra#SemanticsFunction"/>
            </owl:Restriction>
        </rdfs:subClassOf>
        <rdfs:comment>&quot;Given a set of values V = {v1, ..., vm} and their semantics functions f1,...,fm, we propose that the semantics of the set of values in V should be grounded by an aggregation function FV : [−1, 1]m → [−1, 1]. FV takes in the compliance with respect to every individual value and merges them into a single metric. To shorten notation, we denote FV (f1(s), ..., fm(s)) as FV (s).&quot;</rdfs:comment>
        <rdfs:label>SemanticsFunctionAggregation</rdfs:label>
    </owl:Class>
    


    <!-- https://w3id.org/def/vaeontology_montes_sierra#TaxingAgent -->

    <owl:Class rdf:about="https://w3id.org/def/vaeontology_montes_sierra#TaxingAgent">
        <rdfs:subClassOf rdf:resource="https://w3id.org/def/vaeontology#ActingAgent"/>
        <rdfs:subClassOf>
            <owl:Restriction>
                <owl:onProperty rdf:resource="https://w3id.org/def/vaeontology#makesAction"/>
                <owl:allValuesFrom rdf:resource="https://w3id.org/def/vaeontology_montes_sierra#MoneyTransaction"/>
            </owl:Restriction>
        </rdfs:subClassOf>
        <owl:disjointWith rdf:resource="https://w3id.org/def/vaeontology_montes_sierra#TaxingSystem"/>
        <rdfs:comment>&quot;In our running example, the MAS is composed of a set of 200 agents G = {1, 2, ..., 200}. Of these 200, we set 10 to be “evader” agents, which will try to skip payment when the tax collection and redistribution scheme is imposed. This composition of the society (10 out of 200 evader agents) is an arbitrary choice made for exemplification purposes.&quot;</rdfs:comment>
        <rdfs:label>TaxingAgent</rdfs:label>
    </owl:Class>
    


    <!-- https://w3id.org/def/vaeontology_montes_sierra#TaxingAgentState -->

    <owl:Class rdf:about="https://w3id.org/def/vaeontology_montes_sierra#TaxingAgentState">
        <owl:equivalentClass>
            <owl:Restriction>
                <owl:onProperty rdf:resource="https://w3id.org/def/vaeontology#isStateOfAgent"/>
                <owl:someValuesFrom rdf:resource="https://w3id.org/def/vaeontology_montes_sierra#TaxingAgent"/>
            </owl:Restriction>
        </owl:equivalentClass>
        <rdfs:subClassOf rdf:resource="https://w3id.org/def/vaeontology#State"/>
        <rdfs:comment>&quot;At any given time-step, every agent is characterised by its current wealth xi as well as an integer that denotes the wealth segment it belongs to. [...] Therefore, an agent at any state is characterised by the tuple (xi, segi) ∈ (R+ × {1, 2, 3, 4, 5}), where xi is agent i’s wealth (which is always non-negative) and segi is the wealth segment or group it is assigned to&quot;.</rdfs:comment>
        <rdfs:label>TaxingAgentState</rdfs:label>
        <skos:definition>The state of a TaxingAgent.</skos:definition>
    </owl:Class>
    


    <!-- https://w3id.org/def/vaeontology_montes_sierra#TaxingSystem -->

    <owl:Class rdf:about="https://w3id.org/def/vaeontology_montes_sierra#TaxingSystem">
        <rdfs:subClassOf rdf:resource="https://w3id.org/def/vaeontology#System"/>
        <rdfs:comment>&quot;We illustrate all of our contributions with a running example of a toy social model, remi- niscent of the public goods game.&quot;</rdfs:comment>
        <rdfs:label>TaxingSystem</rdfs:label>
        <skos:definition>A class representing a system for the simple taxing example in the paper.</skos:definition>
    </owl:Class>
    


    <!-- https://w3id.org/def/vaeontology_montes_sierra#TaxingSystemState -->

    <owl:Class rdf:about="https://w3id.org/def/vaeontology_montes_sierra#TaxingSystemState">
        <owl:equivalentClass>
            <owl:Restriction>
                <owl:onProperty rdf:resource="https://w3id.org/def/vaeontology#isStateOfAgent"/>
                <owl:someValuesFrom rdf:resource="https://w3id.org/def/vaeontology_montes_sierra#TaxingSystem"/>
            </owl:Restriction>
        </owl:equivalentClass>
        <rdfs:subClassOf rdf:resource="https://w3id.org/def/vaeontology#State"/>
        <rdfs:subClassOf>
            <owl:Restriction>
                <owl:onProperty rdf:resource="http://www.ontologydesignpatterns.org/ont/dul/DUL.owl#hasConstituent"/>
                <owl:minQualifiedCardinality rdf:datatype="http://www.w3.org/2001/XMLSchema#nonNegativeInteger">1</owl:minQualifiedCardinality>
                <owl:onClass rdf:resource="https://w3id.org/def/vaeontology_montes_sierra#TaxingAgentState"/>
            </owl:Restriction>
        </rdfs:subClassOf>
        <rdfs:label>TaxingSystemState</rdfs:label>
        <skos:definition>The state of a TaxingSystem.</skos:definition>
    </owl:Class>
    


    <!-- https://w3id.org/spice/SON/SchwartzValues#SelfTrascendence -->

    <owl:Class rdf:about="https://w3id.org/spice/SON/SchwartzValues#SelfTrascendence"/>
    


    <!-- 
    ///////////////////////////////////////////////////////////////////////////////////////
    //
    // Individuals
    //
    ///////////////////////////////////////////////////////////////////////////////////////
     -->

    


    <!-- https://w3id.org/def/vaeontology_montes_sierra#aggregatedFairnessEqualityOutPath1 -->

    <owl:NamedIndividual rdf:about="https://w3id.org/def/vaeontology_montes_sierra#aggregatedFairnessEqualityOutPath1">
        <rdf:type rdf:resource="https://w3id.org/def/vaeontology_montes_sierra#SemanticsFunctionAggregation"/>
        <dul:hasConstituent rdf:resource="https://w3id.org/def/vaeontology_montes_sierra#equalitySemanticsTaxingOutPath1"/>
        <dul:hasConstituent rdf:resource="https://w3id.org/def/vaeontology_montes_sierra#fairnessSemanticsTaxingOutPath1"/>
        <dul:hasSetting rdf:resource="https://w3id.org/def/vaeontology_montes_sierra#taxProblemContext"/>
        <vae:measuredOnConditionedEntity rdf:resource="https://w3id.org/def/vaeontology_montes_sierra#taxSystemState4"/>
    </owl:NamedIndividual>
    


    <!-- https://w3id.org/def/vaeontology_montes_sierra#alignmentArgumentationOnOptimallyAlignedNormativeSystemsForEquality -->

    <owl:NamedIndividual rdf:about="https://w3id.org/def/vaeontology_montes_sierra#alignmentArgumentationOnOptimallyAlignedNormativeSystemsForEquality">
        <rdf:type rdf:resource="https://w3id.org/def/vaeontology#ArgumentStatement"/>
        <vae:hasClaim rdf:resource="https://w3id.org/def/vaeontology_montes_sierra#optimalAlignmentStatementOnNormativeSystemForEquality"/>
        <vae:hasPremise rdf:resource="https://w3id.org/def/vaeontology_montes_sierra#alignmentStatementOnNormativeSystemForEquality"/>
        <vae:isBasedOnCriterion rdf:resource="https://w3id.org/def/vaeontology_montes_sierra#criterionNormativeSystemAlignment"/>
    </owl:NamedIndividual>
    


    <!-- https://w3id.org/def/vaeontology_montes_sierra#alignmentArgumentationOnOptimallyAlignedNormativeSystemsForFairness -->

    <owl:NamedIndividual rdf:about="https://w3id.org/def/vaeontology_montes_sierra#alignmentArgumentationOnOptimallyAlignedNormativeSystemsForFairness">
        <rdf:type rdf:resource="https://w3id.org/def/vaeontology#ArgumentStatement"/>
        <vae:hasClaim rdf:resource="https://w3id.org/def/vaeontology_montes_sierra#optimalAlignmentStatementOnNormativeSystemForFairness"/>
        <vae:hasPremise rdf:resource="https://w3id.org/def/vaeontology_montes_sierra#alignmentStatementOnNormativeSystemForFairness"/>
        <vae:isBasedOnCriterion rdf:resource="https://w3id.org/def/vaeontology_montes_sierra#criterionNormativeSystemAlignment"/>
    </owl:NamedIndividual>
    


    <!-- https://w3id.org/def/vaeontology_montes_sierra#alignmentPropertyOnNormativeSystemForEquality -->

    <owl:NamedIndividual rdf:about="https://w3id.org/def/vaeontology_montes_sierra#alignmentPropertyOnNormativeSystemForEquality">
        <rdf:type rdf:resource="https://w3id.org/def/vaeontology_montes_sierra#NormativeSystemAlignment"/>
        <vae:measuredOnConditionedEntity rdf:resource="https://w3id.org/def/vaeontology_montes_sierra#taxSystemState2"/>
        <vae:measuredOnConditionedEntity rdf:resource="https://w3id.org/def/vaeontology_montes_sierra#taxSystemState4"/>
        <vae:propertyExpressedAt rdf:resource="https://w3id.org/def/vaeontology_montes_sierra#alignmentStatementOnNormativeSystemForEquality"/>
        <vae:relationWith rdf:resource="https://w3id.org/def/vaeontology_montes_sierra#equalityValueTaxing"/>
        <rdf:value rdf:datatype="http://www.w3.org/2001/XMLSchema#decimal">0.95</rdf:value>
    </owl:NamedIndividual>
    


    <!-- https://w3id.org/def/vaeontology_montes_sierra#alignmentPropertyOnNormativeSystemForFairness -->

    <owl:NamedIndividual rdf:about="https://w3id.org/def/vaeontology_montes_sierra#alignmentPropertyOnNormativeSystemForFairness">
        <rdf:type rdf:resource="https://w3id.org/def/vaeontology_montes_sierra#NormativeSystemAlignment"/>
        <vae:measuredOnConditionedEntity rdf:resource="https://w3id.org/def/vaeontology_montes_sierra#taxSystemState2"/>
        <vae:measuredOnConditionedEntity rdf:resource="https://w3id.org/def/vaeontology_montes_sierra#taxSystemState4"/>
        <vae:propertyExpressedAt rdf:resource="https://w3id.org/def/vaeontology_montes_sierra#alignmentStatementOnNormativeSystemForFairness"/>
        <vae:relationWith rdf:resource="https://w3id.org/def/vaeontology_montes_sierra#fairnessValueTaxing"/>
        <rdf:value rdf:datatype="http://www.w3.org/2001/XMLSchema#decimal">0.93</rdf:value>
    </owl:NamedIndividual>
    


    <!-- https://w3id.org/def/vaeontology_montes_sierra#alignmentStatementOnNormativeSystemForEquality -->

    <owl:NamedIndividual rdf:about="https://w3id.org/def/vaeontology_montes_sierra#alignmentStatementOnNormativeSystemForEquality">
        <rdf:type rdf:resource="https://w3id.org/def/vaeontology#AlignmentStatement"/>
        <vae:interpretationOn rdf:resource="https://w3id.org/def/vaeontology_montes_sierra#equalityValueTaxing"/>
        <vae:onEntity rdf:resource="https://w3id.org/def/vaeontology_montes_sierra#optimizedNormativeSystemForEquality"/>
    </owl:NamedIndividual>
    


    <!-- https://w3id.org/def/vaeontology_montes_sierra#alignmentStatementOnNormativeSystemForFairness -->

    <owl:NamedIndividual rdf:about="https://w3id.org/def/vaeontology_montes_sierra#alignmentStatementOnNormativeSystemForFairness">
        <rdf:type rdf:resource="https://w3id.org/def/vaeontology#AlignmentStatement"/>
        <vae:interpretationOn rdf:resource="https://w3id.org/def/vaeontology_montes_sierra#fairnessValueTaxing"/>
        <vae:onEntity rdf:resource="https://w3id.org/def/vaeontology_montes_sierra#optimizedNormativeSystemForFairness"/>
    </owl:NamedIndividual>
    


    <!-- https://w3id.org/def/vaeontology_montes_sierra#catch -->

    <owl:NamedIndividual rdf:about="https://w3id.org/def/vaeontology_montes_sierra#catch">
        <rdf:type rdf:resource="http://www.ontologydesignpatterns.org/ont/dul/DUL.owl#Parameter"/>
        <hasProbabilityOrFraction rdf:datatype="http://www.w3.org/2001/XMLSchema#decimal">0.44</hasProbabilityOrFraction>
        <rdfs:comment>&quot;Table 1: Optimisation results for the running example with respect to the two values of interest plus their aggregation: optimal normative parameters defining the normative system, and their associated optimal alignment.&quot;</rdfs:comment>
    </owl:NamedIndividual>
    


    <!-- https://w3id.org/def/vaeontology_montes_sierra#catchF -->

    <owl:NamedIndividual rdf:about="https://w3id.org/def/vaeontology_montes_sierra#catchF">
        <rdf:type rdf:resource="http://www.ontologydesignpatterns.org/ont/dul/DUL.owl#Parameter"/>
        <hasProbabilityOrFraction rdf:datatype="http://www.w3.org/2001/XMLSchema#decimal">0.45</hasProbabilityOrFraction>
        <rdfs:comment>&quot;Table 1: Optimisation results for the running example with respect to the two values of interest plus their aggregation: optimal normative parameters defining the normative system, and their associated optimal alignment.&quot;</rdfs:comment>
    </owl:NamedIndividual>
    


    <!-- https://w3id.org/def/vaeontology_montes_sierra#collect -->

    <owl:NamedIndividual rdf:about="https://w3id.org/def/vaeontology_montes_sierra#collect">
        <rdf:type rdf:resource="http://www.ontologydesignpatterns.org/ont/dul/DUL.owl#Parameter"/>
        <dul:hasPart rdf:resource="https://w3id.org/def/vaeontology_montes_sierra#collectSegment1"/>
        <dul:hasPart rdf:resource="https://w3id.org/def/vaeontology_montes_sierra#collectSegment2"/>
        <dul:hasPart rdf:resource="https://w3id.org/def/vaeontology_montes_sierra#collectSegment3"/>
        <dul:hasPart rdf:resource="https://w3id.org/def/vaeontology_montes_sierra#collectSegment4"/>
        <dul:hasPart rdf:resource="https://w3id.org/def/vaeontology_montes_sierra#collectSegment5"/>
        <rdfs:comment>&quot;Table 1: Optimisation results for the running example with respect to the two values of interest plus their aggregation: optimal normative parameters defining the norative system, and their associated optimal alignment.&quot;</rdfs:comment>
    </owl:NamedIndividual>
    


    <!-- https://w3id.org/def/vaeontology_montes_sierra#collectF -->

    <owl:NamedIndividual rdf:about="https://w3id.org/def/vaeontology_montes_sierra#collectF">
        <rdf:type rdf:resource="http://www.ontologydesignpatterns.org/ont/dul/DUL.owl#Parameter"/>
        <dul:hasPart rdf:resource="https://w3id.org/def/vaeontology_montes_sierra#collectFSegment1"/>
        <dul:hasPart rdf:resource="https://w3id.org/def/vaeontology_montes_sierra#collectFSegment2"/>
        <dul:hasPart rdf:resource="https://w3id.org/def/vaeontology_montes_sierra#collectFSegment3"/>
        <dul:hasPart rdf:resource="https://w3id.org/def/vaeontology_montes_sierra#collectFSegment4"/>
        <dul:hasPart rdf:resource="https://w3id.org/def/vaeontology_montes_sierra#collectFSegment5"/>
        <rdfs:comment>&quot;Table 1: Optimisation results for the running example with respect to the two values of interest plus their aggregation: optimal normative parameters defining the norative system, and their associated optimal alignment.&quot;</rdfs:comment>
    </owl:NamedIndividual>
    


    <!-- https://w3id.org/def/vaeontology_montes_sierra#collectFSegment1 -->

    <owl:NamedIndividual rdf:about="https://w3id.org/def/vaeontology_montes_sierra#collectFSegment1">
        <rdf:type rdf:resource="http://www.ontologydesignpatterns.org/ont/dul/DUL.owl#Parameter"/>
        <hasProbabilityOrFraction rdf:datatype="http://www.w3.org/2001/XMLSchema#decimal">0.01</hasProbabilityOrFraction>
        <rdfs:comment>&quot;Table 1: Optimisation results for the running example with respect to the two values of interest plus their aggregation: optimal normative parameters defining the norative system, and their associated optimal alignment.&quot;</rdfs:comment>
    </owl:NamedIndividual>
    


    <!-- https://w3id.org/def/vaeontology_montes_sierra#collectFSegment2 -->

    <owl:NamedIndividual rdf:about="https://w3id.org/def/vaeontology_montes_sierra#collectFSegment2">
        <rdf:type rdf:resource="http://www.ontologydesignpatterns.org/ont/dul/DUL.owl#Parameter"/>
        <hasProbabilityOrFraction rdf:datatype="http://www.w3.org/2001/XMLSchema#decimal">0.30</hasProbabilityOrFraction>
        <rdfs:comment>&quot;Table 1: Optimisation results for the running example with respect to the two values of interest plus their aggregation: optimal normative parameters defining the norative system, and their associated optimal alignment.&quot;</rdfs:comment>
    </owl:NamedIndividual>
    


    <!-- https://w3id.org/def/vaeontology_montes_sierra#collectFSegment3 -->

    <owl:NamedIndividual rdf:about="https://w3id.org/def/vaeontology_montes_sierra#collectFSegment3">
        <rdf:type rdf:resource="http://www.ontologydesignpatterns.org/ont/dul/DUL.owl#Parameter"/>
        <hasProbabilityOrFraction rdf:datatype="http://www.w3.org/2001/XMLSchema#decimal">0.37</hasProbabilityOrFraction>
        <rdfs:comment>&quot;Table 1: Optimisation results for the running example with respect to the two values of interest plus their aggregation: optimal normative parameters defining the norative system, and their associated optimal alignment.&quot;</rdfs:comment>
    </owl:NamedIndividual>
    


    <!-- https://w3id.org/def/vaeontology_montes_sierra#collectFSegment4 -->

    <owl:NamedIndividual rdf:about="https://w3id.org/def/vaeontology_montes_sierra#collectFSegment4">
        <rdf:type rdf:resource="http://www.ontologydesignpatterns.org/ont/dul/DUL.owl#Parameter"/>
        <hasProbabilityOrFraction rdf:datatype="http://www.w3.org/2001/XMLSchema#decimal">0.72</hasProbabilityOrFraction>
        <rdfs:comment>&quot;Table 1: Optimisation results for the running example with respect to the two values of interest plus their aggregation: optimal normative parameters defining the norative system, and their associated optimal alignment.&quot;</rdfs:comment>
    </owl:NamedIndividual>
    


    <!-- https://w3id.org/def/vaeontology_montes_sierra#collectFSegment5 -->

    <owl:NamedIndividual rdf:about="https://w3id.org/def/vaeontology_montes_sierra#collectFSegment5">
        <rdf:type rdf:resource="http://www.ontologydesignpatterns.org/ont/dul/DUL.owl#Parameter"/>
        <hasProbabilityOrFraction rdf:datatype="http://www.w3.org/2001/XMLSchema#decimal">0.66</hasProbabilityOrFraction>
        <rdfs:comment>&quot;Table 1: Optimisation results for the running example with respect to the two values of interest plus their aggregation: optimal normative parameters defining the norative system, and their associated optimal alignment.&quot;</rdfs:comment>
    </owl:NamedIndividual>
    


    <!-- https://w3id.org/def/vaeontology_montes_sierra#collectSegment1 -->

    <owl:NamedIndividual rdf:about="https://w3id.org/def/vaeontology_montes_sierra#collectSegment1">
        <rdf:type rdf:resource="http://www.ontologydesignpatterns.org/ont/dul/DUL.owl#Parameter"/>
        <hasProbabilityOrFraction rdf:datatype="http://www.w3.org/2001/XMLSchema#decimal">0.2</hasProbabilityOrFraction>
        <rdfs:comment>&quot;Table 1: Optimisation results for the running example with respect to the two values of interest plus their aggregation: optimal normative parameters defining the norative system, and their associated optimal alignment.&quot;</rdfs:comment>
    </owl:NamedIndividual>
    


    <!-- https://w3id.org/def/vaeontology_montes_sierra#collectSegment2 -->

    <owl:NamedIndividual rdf:about="https://w3id.org/def/vaeontology_montes_sierra#collectSegment2">
        <rdf:type rdf:resource="http://www.ontologydesignpatterns.org/ont/dul/DUL.owl#Parameter"/>
        <hasProbabilityOrFraction rdf:datatype="http://www.w3.org/2001/XMLSchema#decimal">0.29</hasProbabilityOrFraction>
        <rdfs:comment>&quot;Table 1: Optimisation results for the running example with respect to the two values of interest plus their aggregation: optimal normative parameters defining the norative system, and their associated optimal alignment.&quot;</rdfs:comment>
    </owl:NamedIndividual>
    


    <!-- https://w3id.org/def/vaeontology_montes_sierra#collectSegment3 -->

    <owl:NamedIndividual rdf:about="https://w3id.org/def/vaeontology_montes_sierra#collectSegment3">
        <rdf:type rdf:resource="http://www.ontologydesignpatterns.org/ont/dul/DUL.owl#Parameter"/>
        <hasProbabilityOrFraction rdf:datatype="http://www.w3.org/2001/XMLSchema#decimal">0.26</hasProbabilityOrFraction>
        <rdfs:comment>&quot;Table 1: Optimisation results for the running example with respect to the two values of interest plus their aggregation: optimal normative parameters defining the norative system, and their associated optimal alignment.&quot;</rdfs:comment>
    </owl:NamedIndividual>
    


    <!-- https://w3id.org/def/vaeontology_montes_sierra#collectSegment4 -->

    <owl:NamedIndividual rdf:about="https://w3id.org/def/vaeontology_montes_sierra#collectSegment4">
        <rdf:type rdf:resource="http://www.ontologydesignpatterns.org/ont/dul/DUL.owl#Parameter"/>
        <hasProbabilityOrFraction rdf:datatype="http://www.w3.org/2001/XMLSchema#decimal">0.35</hasProbabilityOrFraction>
        <rdfs:comment>&quot;Table 1: Optimisation results for the running example with respect to the two values of interest plus their aggregation: optimal normative parameters defining the norative system, and their associated optimal alignment.&quot;</rdfs:comment>
    </owl:NamedIndividual>
    


    <!-- https://w3id.org/def/vaeontology_montes_sierra#collectSegment5 -->

    <owl:NamedIndividual rdf:about="https://w3id.org/def/vaeontology_montes_sierra#collectSegment5">
        <rdf:type rdf:resource="http://www.ontologydesignpatterns.org/ont/dul/DUL.owl#Parameter"/>
        <hasProbabilityOrFraction rdf:datatype="http://www.w3.org/2001/XMLSchema#decimal">0.27</hasProbabilityOrFraction>
        <rdfs:comment>&quot;Table 1: Optimisation results for the running example with respect to the two values of interest plus their aggregation: optimal normative parameters defining the norative system, and their associated optimal alignment.&quot;</rdfs:comment>
    </owl:NamedIndividual>
    


    <!-- https://w3id.org/def/vaeontology_montes_sierra#criterionNormativeSystemAlignment -->

    <owl:NamedIndividual rdf:about="https://w3id.org/def/vaeontology_montes_sierra#criterionNormativeSystemAlignment">
        <rdf:type rdf:resource="https://w3id.org/def/vaeontology#Criterion"/>
        <dul:hasSetting rdf:resource="https://w3id.org/def/vaeontology_montes_sierra#taxProblemContext"/>
        <odrl:constraint rdf:resource="https://w3id.org/def/vaeontology_montes_sierra#targetPropertyOptimizedAtAction"/>
        <vae:interpretationOn rdf:resource="https://w3id.org/def/vaeontology_montes_sierra#equalityValueTaxing"/>
        <vae:interpretationOn rdf:resource="https://w3id.org/def/vaeontology_montes_sierra#fairnessValueTaxing"/>
    </owl:NamedIndividual>
    


    <!-- https://w3id.org/def/vaeontology_montes_sierra#equalitySemanticsTaxingOutPath1 -->

    <owl:NamedIndividual rdf:about="https://w3id.org/def/vaeontology_montes_sierra#equalitySemanticsTaxingOutPath1">
        <rdf:type rdf:resource="https://w3id.org/def/vaeontology_montes_sierra#GiniIndex"/>
        <dul:hasSetting rdf:resource="https://w3id.org/def/vaeontology_montes_sierra#taxProblemContext"/>
        <vae:measuredOnConditionedEntity rdf:resource="https://w3id.org/def/vaeontology_montes_sierra#taxSystemState4"/>
        <rdfs:comment>&quot;First, we ground the meaning of value equality in the context of our model as, of course, economic equality. To do so, we use the well-known Gini index indicator (Gini, 1912), a widespread metric to quantify wealth and income inequality (The World Bank, Development Research Group, 2019)&quot;</rdfs:comment>
        <rdfs:label>&quot;Gini Index-based semantics function&quot;</rdfs:label>
    </owl:NamedIndividual>
    


    <!-- https://w3id.org/def/vaeontology_montes_sierra#equalityValueTaxing -->

    <owl:NamedIndividual rdf:about="https://w3id.org/def/vaeontology_montes_sierra#equalityValueTaxing">
        <rdf:type rdf:resource="https://w3id.org/def/vaeontology#Equality"/>
        <dul:hasSetting rdf:resource="https://w3id.org/def/vaeontology_montes_sierra#taxProblemContext"/>
        <rdfs:label>equalityValueTaxing</rdfs:label>
    </owl:NamedIndividual>
    


    <!-- https://w3id.org/def/vaeontology_montes_sierra#evaderAgent1 -->

    <owl:NamedIndividual rdf:about="https://w3id.org/def/vaeontology_montes_sierra#evaderAgent1">
        <rdf:type rdf:resource="https://w3id.org/def/vaeontology_montes_sierra#EvaderAgent"/>
        <dul:hasSetting rdf:resource="https://w3id.org/def/vaeontology_montes_sierra#taxProblemContext"/>
        <vae:isAgentOfSystem rdf:resource="https://w3id.org/def/vaeontology_montes_sierra#taxingSystem"/>
    </owl:NamedIndividual>
    


    <!-- https://w3id.org/def/vaeontology_montes_sierra#evaderAgent1State1 -->

    <owl:NamedIndividual rdf:about="https://w3id.org/def/vaeontology_montes_sierra#evaderAgent1State1">
        <rdf:type rdf:resource="https://w3id.org/def/vaeontology_montes_sierra#TaxingAgentState"/>
        <dul:hasSetting rdf:resource="https://w3id.org/def/vaeontology_montes_sierra#taxProblemContext"/>
        <vae:isStateOfAgent rdf:resource="https://w3id.org/def/vaeontology_montes_sierra#evaderAgent1"/>
        <belongsToSegment rdf:datatype="http://www.w3.org/2001/XMLSchema#decimal">3</belongsToSegment>
        <hasWealth rdf:datatype="http://www.w3.org/2001/XMLSchema#decimal">57</hasWealth>
    </owl:NamedIndividual>
    


    <!-- https://w3id.org/def/vaeontology_montes_sierra#evaderAgent1State2 -->

    <owl:NamedIndividual rdf:about="https://w3id.org/def/vaeontology_montes_sierra#evaderAgent1State2">
        <rdf:type rdf:resource="https://w3id.org/def/vaeontology_montes_sierra#TaxingAgentState"/>
        <dul:hasSetting rdf:resource="https://w3id.org/def/vaeontology_montes_sierra#taxProblemContext"/>
        <vae:isStateOfAgent rdf:resource="https://w3id.org/def/vaeontology_montes_sierra#evaderAgent1"/>
        <belongsToSegment rdf:datatype="http://www.w3.org/2001/XMLSchema#decimal">4</belongsToSegment>
        <hasWealth rdf:datatype="http://www.w3.org/2001/XMLSchema#decimal">76</hasWealth>
    </owl:NamedIndividual>
    


    <!-- https://w3id.org/def/vaeontology_montes_sierra#evaderAgent1State3 -->

    <owl:NamedIndividual rdf:about="https://w3id.org/def/vaeontology_montes_sierra#evaderAgent1State3">
        <rdf:type rdf:resource="https://w3id.org/def/vaeontology_montes_sierra#TaxingAgentState"/>
        <dul:hasSetting rdf:resource="https://w3id.org/def/vaeontology_montes_sierra#taxProblemContext"/>
        <vae:isStateOfAgent rdf:resource="https://w3id.org/def/vaeontology_montes_sierra#evaderAgent1"/>
        <belongsToSegment rdf:datatype="http://www.w3.org/2001/XMLSchema#decimal">2</belongsToSegment>
        <hasWealth rdf:datatype="http://www.w3.org/2001/XMLSchema#decimal">16</hasWealth>
    </owl:NamedIndividual>
    


    <!-- https://w3id.org/def/vaeontology_montes_sierra#evaderAgent1State4 -->

    <owl:NamedIndividual rdf:about="https://w3id.org/def/vaeontology_montes_sierra#evaderAgent1State4">
        <rdf:type rdf:resource="https://w3id.org/def/vaeontology_montes_sierra#TaxingAgentState"/>
        <dul:hasSetting rdf:resource="https://w3id.org/def/vaeontology_montes_sierra#taxProblemContext"/>
        <vae:isStateOfAgent rdf:resource="https://w3id.org/def/vaeontology_montes_sierra#evaderAgent1"/>
        <belongsToSegment rdf:datatype="http://www.w3.org/2001/XMLSchema#decimal">1</belongsToSegment>
        <hasWealth rdf:datatype="http://www.w3.org/2001/XMLSchema#decimal">0</hasWealth>
    </owl:NamedIndividual>
    


    <!-- https://w3id.org/def/vaeontology_montes_sierra#fairnessSemanticsTaxingOutPath1 -->

    <owl:NamedIndividual rdf:about="https://w3id.org/def/vaeontology_montes_sierra#fairnessSemanticsTaxingOutPath1">
        <rdf:type rdf:resource="https://w3id.org/def/vaeontology_montes_sierra#ProbabilityTaxFairnessSemantics"/>
        <dul:hasSetting rdf:resource="https://w3id.org/def/vaeontology_montes_sierra#taxProblemContext"/>
        <vae:measuredOnConditionedEntity rdf:resource="https://w3id.org/def/vaeontology_montes_sierra#taxSystemState4"/>
        <rdfs:comment>&quot;Second, we ground the semantics of value fairness to mean that evader individuals should be punished for their evasion. Hence, we consider that fairness is being highly promoted if, by the end of a fixed-length path, as many evaders as possible belong to the poorest wealth segment&quot;</rdfs:comment>
    </owl:NamedIndividual>
    


    <!-- https://w3id.org/def/vaeontology_montes_sierra#fairnessValueTaxing -->

    <owl:NamedIndividual rdf:about="https://w3id.org/def/vaeontology_montes_sierra#fairnessValueTaxing">
        <rdf:type rdf:resource="https://w3id.org/def/vaeontology_montes_sierra#Fairness"/>
        <dul:hasSetting rdf:resource="https://w3id.org/def/vaeontology_montes_sierra#taxProblemContext"/>
        <rdfs:label>fairnessValueTaxing</rdfs:label>
    </owl:NamedIndividual>
    


    <!-- https://w3id.org/def/vaeontology_montes_sierra#fine -->

    <owl:NamedIndividual rdf:about="https://w3id.org/def/vaeontology_montes_sierra#fine">
        <rdf:type rdf:resource="http://www.ontologydesignpatterns.org/ont/dul/DUL.owl#Parameter"/>
        <hasProbabilityOrFraction rdf:datatype="http://www.w3.org/2001/XMLSchema#decimal">0.61</hasProbabilityOrFraction>
    </owl:NamedIndividual>
    


    <!-- https://w3id.org/def/vaeontology_montes_sierra#fineF -->

    <owl:NamedIndividual rdf:about="https://w3id.org/def/vaeontology_montes_sierra#fineF">
        <rdf:type rdf:resource="http://www.ontologydesignpatterns.org/ont/dul/DUL.owl#Parameter"/>
        <hasProbabilityOrFraction rdf:datatype="http://www.w3.org/2001/XMLSchema#decimal">0.56</hasProbabilityOrFraction>
    </owl:NamedIndividual>
    


    <!-- https://w3id.org/def/vaeontology_montes_sierra#jointMoneyTransaction -->

    <owl:NamedIndividual rdf:about="https://w3id.org/def/vaeontology_montes_sierra#jointMoneyTransaction">
        <rdf:type rdf:resource="https://w3id.org/def/vaeontology#Action"/>
        <dul:hasParticipant rdf:resource="https://w3id.org/def/vaeontology_montes_sierra#evaderAgent1"/>
        <dul:hasParticipant rdf:resource="https://w3id.org/def/vaeontology_montes_sierra#payerAgent1"/>
        <dul:hasSetting rdf:resource="https://w3id.org/def/vaeontology_montes_sierra#taxProblemContext"/>
        <vae:composedBySequence rdf:resource="https://w3id.org/def/vaeontology_montes_sierra#taxSystemActionSequence"/>
        <vae:isInputOf rdf:resource="https://w3id.org/def/vaeontology_montes_sierra#path1transition1"/>
    </owl:NamedIndividual>
    


    <!-- https://w3id.org/def/vaeontology_montes_sierra#operatorIsOptimizedAt -->

    <owl:NamedIndividual rdf:about="https://w3id.org/def/vaeontology_montes_sierra#operatorIsOptimizedAt">
        <rdf:value>premise expressesProperty that vae:isPropertyOptimizedAt B, which vae:propertyExpressedAt claim</rdf:value>
    </owl:NamedIndividual>
    


    <!-- https://w3id.org/def/vaeontology_montes_sierra#optimalAlignmentPropertyOnNormativeSystemForEquality -->

    <owl:NamedIndividual rdf:about="https://w3id.org/def/vaeontology_montes_sierra#optimalAlignmentPropertyOnNormativeSystemForEquality">
        <rdf:type rdf:resource="https://w3id.org/def/vaeontology_montes_sierra#OptimalNormativeSystemAlignment"/>
        <dul:hasSetting rdf:resource="https://w3id.org/def/vaeontology_montes_sierra#taxProblemContext"/>
        <vae:isOptimizationOfProperty rdf:resource="https://w3id.org/def/vaeontology_montes_sierra#alignmentPropertyOnNormativeSystemForEquality"/>
        <vae:measuredOnConditionedEntity rdf:resource="https://w3id.org/def/vaeontology_montes_sierra#taxSystemPath1"/>
        <vae:measuredOnConditionedEntity rdf:resource="https://w3id.org/def/vaeontology_montes_sierra#taxSystemPath2"/>
        <vae:measuredOnConditionedEntity rdf:resource="https://w3id.org/def/vaeontology_montes_sierra#taxSystemState2"/>
        <vae:measuredOnConditionedEntity rdf:resource="https://w3id.org/def/vaeontology_montes_sierra#taxSystemState4"/>
        <vae:propertyExpressedAt rdf:resource="https://w3id.org/def/vaeontology_montes_sierra#optimalAlignmentStatementOnNormativeSystemForEquality"/>
        <rdf:value rdf:datatype="http://www.w3.org/2001/XMLSchema#decimal">0.95</rdf:value>
    </owl:NamedIndividual>
    


    <!-- https://w3id.org/def/vaeontology_montes_sierra#optimalAlignmentPropertyOnNormativeSystemForFairness -->

    <owl:NamedIndividual rdf:about="https://w3id.org/def/vaeontology_montes_sierra#optimalAlignmentPropertyOnNormativeSystemForFairness">
        <rdf:type rdf:resource="https://w3id.org/def/vaeontology_montes_sierra#OptimalNormativeSystemAlignment"/>
        <dul:hasSetting rdf:resource="https://w3id.org/def/vaeontology_montes_sierra#taxProblemContext"/>
        <vae:isOptimizationOfProperty rdf:resource="https://w3id.org/def/vaeontology_montes_sierra#alignmentPropertyOnNormativeSystemForFairness"/>
        <vae:measuredOnConditionedEntity rdf:resource="https://w3id.org/def/vaeontology_montes_sierra#taxSystemPath1"/>
        <vae:measuredOnConditionedEntity rdf:resource="https://w3id.org/def/vaeontology_montes_sierra#taxSystemPath2"/>
        <vae:measuredOnConditionedEntity rdf:resource="https://w3id.org/def/vaeontology_montes_sierra#taxSystemState2"/>
        <vae:measuredOnConditionedEntity rdf:resource="https://w3id.org/def/vaeontology_montes_sierra#taxSystemState4"/>
        <vae:propertyExpressedAt rdf:resource="https://w3id.org/def/vaeontology_montes_sierra#optimalAlignmentStatementOnNormativeSystemForFairness"/>
        <rdf:value rdf:datatype="http://www.w3.org/2001/XMLSchema#decimal">0.93</rdf:value>
    </owl:NamedIndividual>
    


    <!-- https://w3id.org/def/vaeontology_montes_sierra#optimalAlignmentStatementOnNormativeSystemForEquality -->

    <owl:NamedIndividual rdf:about="https://w3id.org/def/vaeontology_montes_sierra#optimalAlignmentStatementOnNormativeSystemForEquality">
        <rdf:type rdf:resource="https://w3id.org/def/vaeontology#AlignmentStatement"/>
        <dul:hasSetting rdf:resource="https://w3id.org/def/vaeontology_montes_sierra#taxProblemContext"/>
        <vae:interpretationOn rdf:resource="https://w3id.org/def/vaeontology_montes_sierra#equalityValueTaxing"/>
        <vae:onEntity rdf:resource="https://w3id.org/def/vaeontology_montes_sierra#optimizedNormativeSystemForEquality"/>
    </owl:NamedIndividual>
    


    <!-- https://w3id.org/def/vaeontology_montes_sierra#optimalAlignmentStatementOnNormativeSystemForFairness -->

    <owl:NamedIndividual rdf:about="https://w3id.org/def/vaeontology_montes_sierra#optimalAlignmentStatementOnNormativeSystemForFairness">
        <rdf:type rdf:resource="https://w3id.org/def/vaeontology#AlignmentStatement"/>
        <dul:hasSetting rdf:resource="https://w3id.org/def/vaeontology_montes_sierra#taxProblemContext"/>
        <vae:interpretationOn rdf:resource="https://w3id.org/def/vaeontology_montes_sierra#fairnessValueTaxing"/>
        <vae:onEntity rdf:resource="https://w3id.org/def/vaeontology_montes_sierra#optimizedNormativeSystemForFairness"/>
    </owl:NamedIndividual>
    


    <!-- https://w3id.org/def/vaeontology_montes_sierra#optimizedNormativeSystemForEquality -->

    <owl:NamedIndividual rdf:about="https://w3id.org/def/vaeontology_montes_sierra#optimizedNormativeSystemForEquality">
        <rdf:type rdf:resource="https://w3id.org/def/vaeontology_montes_sierra#NormativeSystem"/>
        <dul:hasParameter rdf:resource="https://w3id.org/def/vaeontology_montes_sierra#catch"/>
        <dul:hasParameter rdf:resource="https://w3id.org/def/vaeontology_montes_sierra#collect"/>
        <dul:hasParameter rdf:resource="https://w3id.org/def/vaeontology_montes_sierra#fine"/>
        <dul:hasParameter rdf:resource="https://w3id.org/def/vaeontology_montes_sierra#redistribute"/>
        <dul:hasSetting rdf:resource="https://w3id.org/def/vaeontology_montes_sierra#taxProblemContext"/>
        <odrl:assignee rdf:resource="https://w3id.org/def/vaeontology_montes_sierra#evaderAgent1"/>
        <odrl:assignee rdf:resource="https://w3id.org/def/vaeontology_montes_sierra#payerAgent1"/>
        <odrl:assigner rdf:resource="https://w3id.org/def/vaeontology_montes_sierra#problemModeller"/>
        <odrl:target rdf:resource="https://w3id.org/def/vaeontology_montes_sierra#taxingSystem"/>
        <vae:influencesOutcome rdf:resource="https://w3id.org/def/vaeontology_montes_sierra#taxSystemPath1"/>
        <vae:influencesOutcome rdf:resource="https://w3id.org/def/vaeontology_montes_sierra#taxSystemPath2"/>
        <vae:influencesOutcome rdf:resource="https://w3id.org/def/vaeontology_montes_sierra#transactionPayingTaxes"/>
        <vae:reflectsValue rdf:resource="https://w3id.org/def/vaeontology_montes_sierra#equalityValueTaxing"/>
    </owl:NamedIndividual>
    


    <!-- https://w3id.org/def/vaeontology_montes_sierra#optimizedNormativeSystemForFairness -->

    <owl:NamedIndividual rdf:about="https://w3id.org/def/vaeontology_montes_sierra#optimizedNormativeSystemForFairness">
        <rdf:type rdf:resource="https://w3id.org/def/vaeontology_montes_sierra#NormativeSystem"/>
        <dul:hasParameter rdf:resource="https://w3id.org/def/vaeontology_montes_sierra#catchF"/>
        <dul:hasParameter rdf:resource="https://w3id.org/def/vaeontology_montes_sierra#collectF"/>
        <dul:hasParameter rdf:resource="https://w3id.org/def/vaeontology_montes_sierra#fineF"/>
        <dul:hasParameter rdf:resource="https://w3id.org/def/vaeontology_montes_sierra#redistributeF"/>
        <dul:hasSetting rdf:resource="https://w3id.org/def/vaeontology_montes_sierra#taxProblemContext"/>
        <odrl:assignee rdf:resource="https://w3id.org/def/vaeontology_montes_sierra#evaderAgent1"/>
        <odrl:assignee rdf:resource="https://w3id.org/def/vaeontology_montes_sierra#payerAgent1"/>
        <odrl:assigner rdf:resource="https://w3id.org/def/vaeontology_montes_sierra#problemModeller"/>
        <odrl:target rdf:resource="https://w3id.org/def/vaeontology_montes_sierra#taxingSystem"/>
        <vae:influencesOutcome rdf:resource="https://w3id.org/def/vaeontology_montes_sierra#taxSystemPath1"/>
        <vae:influencesOutcome rdf:resource="https://w3id.org/def/vaeontology_montes_sierra#taxSystemPath2"/>
        <vae:influencesOutcome rdf:resource="https://w3id.org/def/vaeontology_montes_sierra#transactionPayingTaxes"/>
        <vae:reflectsValue rdf:resource="https://w3id.org/def/vaeontology_montes_sierra#fairnessValueTaxing"/>
    </owl:NamedIndividual>
    


    <!-- https://w3id.org/def/vaeontology_montes_sierra#parametricNorm1_eq -->

    <owl:NamedIndividual rdf:about="https://w3id.org/def/vaeontology_montes_sierra#parametricNorm1_eq">
        <rdf:type rdf:resource="https://w3id.org/def/vaeontology_montes_sierra#ParametricNorm"/>
        <dul:hasParameter rdf:resource="https://w3id.org/def/vaeontology_montes_sierra#collect"/>
        <dul:hasSetting rdf:resource="https://w3id.org/def/vaeontology_montes_sierra#taxProblemContext"/>
        <dul:isMemberOf rdf:resource="https://w3id.org/def/vaeontology_montes_sierra#optimizedNormativeSystemForEquality"/>
        <odrl:assignee rdf:resource="https://w3id.org/def/vaeontology_montes_sierra#evaderAgent1"/>
        <odrl:assignee rdf:resource="https://w3id.org/def/vaeontology_montes_sierra#payerAgent1"/>
        <odrl:assigner rdf:resource="https://w3id.org/def/vaeontology_montes_sierra#problemModeller"/>
        <odrl:target rdf:resource="https://w3id.org/def/vaeontology_montes_sierra#taxingSystem"/>
    </owl:NamedIndividual>
    


    <!-- https://w3id.org/def/vaeontology_montes_sierra#parametricNorm1_fair -->

    <owl:NamedIndividual rdf:about="https://w3id.org/def/vaeontology_montes_sierra#parametricNorm1_fair">
        <rdf:type rdf:resource="https://w3id.org/def/vaeontology_montes_sierra#ParametricNorm"/>
        <dul:hasParameter rdf:resource="https://w3id.org/def/vaeontology_montes_sierra#collectF"/>
        <dul:hasSetting rdf:resource="https://w3id.org/def/vaeontology_montes_sierra#taxProblemContext"/>
        <dul:isMemberOf rdf:resource="https://w3id.org/def/vaeontology_montes_sierra#optimizedNormativeSystemForFairness"/>
        <odrl:assignee rdf:resource="https://w3id.org/def/vaeontology_montes_sierra#evaderAgent1"/>
        <odrl:assignee rdf:resource="https://w3id.org/def/vaeontology_montes_sierra#payerAgent1"/>
        <odrl:assigner rdf:resource="https://w3id.org/def/vaeontology_montes_sierra#problemModeller"/>
        <odrl:target rdf:resource="https://w3id.org/def/vaeontology_montes_sierra#taxingSystem"/>
    </owl:NamedIndividual>
    


    <!-- https://w3id.org/def/vaeontology_montes_sierra#parametricNorm2_eq -->

    <owl:NamedIndividual rdf:about="https://w3id.org/def/vaeontology_montes_sierra#parametricNorm2_eq">
        <rdf:type rdf:resource="https://w3id.org/def/vaeontology_montes_sierra#ParametricNorm"/>
        <dul:hasParameter rdf:resource="https://w3id.org/def/vaeontology_montes_sierra#redistribute"/>
        <dul:hasSetting rdf:resource="https://w3id.org/def/vaeontology_montes_sierra#taxProblemContext"/>
        <dul:isMemberOf rdf:resource="https://w3id.org/def/vaeontology_montes_sierra#optimizedNormativeSystemForEquality"/>
        <odrl:assignee rdf:resource="https://w3id.org/def/vaeontology_montes_sierra#evaderAgent1"/>
        <odrl:assignee rdf:resource="https://w3id.org/def/vaeontology_montes_sierra#payerAgent1"/>
        <odrl:assigner rdf:resource="https://w3id.org/def/vaeontology_montes_sierra#problemModeller"/>
        <odrl:target rdf:resource="https://w3id.org/def/vaeontology_montes_sierra#taxingSystem"/>
    </owl:NamedIndividual>
    


    <!-- https://w3id.org/def/vaeontology_montes_sierra#parametricNorm2_fair -->

    <owl:NamedIndividual rdf:about="https://w3id.org/def/vaeontology_montes_sierra#parametricNorm2_fair">
        <rdf:type rdf:resource="https://w3id.org/def/vaeontology_montes_sierra#ParametricNorm"/>
        <dul:hasParameter rdf:resource="https://w3id.org/def/vaeontology_montes_sierra#redistributeF"/>
        <dul:hasSetting rdf:resource="https://w3id.org/def/vaeontology_montes_sierra#taxProblemContext"/>
        <dul:isMemberOf rdf:resource="https://w3id.org/def/vaeontology_montes_sierra#optimizedNormativeSystemForFairness"/>
        <odrl:assignee rdf:resource="https://w3id.org/def/vaeontology_montes_sierra#evaderAgent1"/>
        <odrl:assignee rdf:resource="https://w3id.org/def/vaeontology_montes_sierra#payerAgent1"/>
        <odrl:assigner rdf:resource="https://w3id.org/def/vaeontology_montes_sierra#problemModeller"/>
        <odrl:target rdf:resource="https://w3id.org/def/vaeontology_montes_sierra#taxingSystem"/>
    </owl:NamedIndividual>
    


    <!-- https://w3id.org/def/vaeontology_montes_sierra#parametricNorm3_eq -->

    <owl:NamedIndividual rdf:about="https://w3id.org/def/vaeontology_montes_sierra#parametricNorm3_eq">
        <rdf:type rdf:resource="https://w3id.org/def/vaeontology_montes_sierra#ParametricNorm"/>
        <dul:hasParameter rdf:resource="https://w3id.org/def/vaeontology_montes_sierra#catch"/>
        <dul:hasSetting rdf:resource="https://w3id.org/def/vaeontology_montes_sierra#taxProblemContext"/>
        <dul:isMemberOf rdf:resource="https://w3id.org/def/vaeontology_montes_sierra#optimizedNormativeSystemForEquality"/>
        <odrl:assignee rdf:resource="https://w3id.org/def/vaeontology_montes_sierra#evaderAgent1"/>
        <odrl:assignee rdf:resource="https://w3id.org/def/vaeontology_montes_sierra#payerAgent1"/>
        <odrl:assigner rdf:resource="https://w3id.org/def/vaeontology_montes_sierra#problemModeller"/>
        <odrl:target rdf:resource="https://w3id.org/def/vaeontology_montes_sierra#taxingSystem"/>
    </owl:NamedIndividual>
    


    <!-- https://w3id.org/def/vaeontology_montes_sierra#parametricNorm3_fair -->

    <owl:NamedIndividual rdf:about="https://w3id.org/def/vaeontology_montes_sierra#parametricNorm3_fair">
        <rdf:type rdf:resource="https://w3id.org/def/vaeontology_montes_sierra#ParametricNorm"/>
        <dul:hasParameter rdf:resource="https://w3id.org/def/vaeontology_montes_sierra#catchF"/>
        <dul:hasSetting rdf:resource="https://w3id.org/def/vaeontology_montes_sierra#taxProblemContext"/>
        <dul:isMemberOf rdf:resource="https://w3id.org/def/vaeontology_montes_sierra#optimizedNormativeSystemForFairness"/>
        <odrl:assignee rdf:resource="https://w3id.org/def/vaeontology_montes_sierra#evaderAgent1"/>
        <odrl:assignee rdf:resource="https://w3id.org/def/vaeontology_montes_sierra#payerAgent1"/>
        <odrl:assigner rdf:resource="https://w3id.org/def/vaeontology_montes_sierra#problemModeller"/>
        <odrl:target rdf:resource="https://w3id.org/def/vaeontology_montes_sierra#taxingSystem"/>
    </owl:NamedIndividual>
    


    <!-- https://w3id.org/def/vaeontology_montes_sierra#parametricNorm4_eq -->

    <owl:NamedIndividual rdf:about="https://w3id.org/def/vaeontology_montes_sierra#parametricNorm4_eq">
        <rdf:type rdf:resource="https://w3id.org/def/vaeontology_montes_sierra#ParametricNorm"/>
        <dul:hasParameter rdf:resource="https://w3id.org/def/vaeontology_montes_sierra#fine"/>
        <dul:hasSetting rdf:resource="https://w3id.org/def/vaeontology_montes_sierra#taxProblemContext"/>
        <dul:isMemberOf rdf:resource="https://w3id.org/def/vaeontology_montes_sierra#optimizedNormativeSystemForEquality"/>
        <odrl:assignee rdf:resource="https://w3id.org/def/vaeontology_montes_sierra#evaderAgent1"/>
        <odrl:assignee rdf:resource="https://w3id.org/def/vaeontology_montes_sierra#payerAgent1"/>
        <odrl:assigner rdf:resource="https://w3id.org/def/vaeontology_montes_sierra#problemModeller"/>
        <odrl:target rdf:resource="https://w3id.org/def/vaeontology_montes_sierra#taxingSystem"/>
    </owl:NamedIndividual>
    


    <!-- https://w3id.org/def/vaeontology_montes_sierra#parametricNorm4_fair -->

    <owl:NamedIndividual rdf:about="https://w3id.org/def/vaeontology_montes_sierra#parametricNorm4_fair">
        <rdf:type rdf:resource="https://w3id.org/def/vaeontology_montes_sierra#ParametricNorm"/>
        <dul:hasParameter rdf:resource="https://w3id.org/def/vaeontology_montes_sierra#fineF"/>
        <dul:hasSetting rdf:resource="https://w3id.org/def/vaeontology_montes_sierra#taxProblemContext"/>
        <dul:isMemberOf rdf:resource="https://w3id.org/def/vaeontology_montes_sierra#optimizedNormativeSystemForFairness"/>
        <odrl:assignee rdf:resource="https://w3id.org/def/vaeontology_montes_sierra#evaderAgent1"/>
        <odrl:assignee rdf:resource="https://w3id.org/def/vaeontology_montes_sierra#payerAgent1"/>
        <odrl:assigner rdf:resource="https://w3id.org/def/vaeontology_montes_sierra#problemModeller"/>
        <odrl:target rdf:resource="https://w3id.org/def/vaeontology_montes_sierra#taxingSystem"/>
    </owl:NamedIndividual>
    


    <!-- https://w3id.org/def/vaeontology_montes_sierra#path1transition1 -->

    <owl:NamedIndividual rdf:about="https://w3id.org/def/vaeontology_montes_sierra#path1transition1">
        <rdf:type rdf:resource="https://w3id.org/def/vaeontology#Transition"/>
        <dul:hasSetting rdf:resource="https://w3id.org/def/vaeontology_montes_sierra#taxProblemContext"/>
        <vae:hasInput rdf:resource="https://w3id.org/def/vaeontology_montes_sierra#jointMoneyTransaction"/>
        <vae:hasInput rdf:resource="https://w3id.org/def/vaeontology_montes_sierra#taxSystemState1"/>
        <vae:hasOutcome rdf:resource="https://w3id.org/def/vaeontology_montes_sierra#taxSystemState2"/>
        <vae:nextInputOutcome rdf:resource="https://w3id.org/def/vaeontology_montes_sierra#path1transition2"/>
    </owl:NamedIndividual>
    


    <!-- https://w3id.org/def/vaeontology_montes_sierra#path1transition2 -->

    <owl:NamedIndividual rdf:about="https://w3id.org/def/vaeontology_montes_sierra#path1transition2">
        <rdf:type rdf:resource="https://w3id.org/def/vaeontology#Transition"/>
        <dul:hasSetting rdf:resource="https://w3id.org/def/vaeontology_montes_sierra#taxProblemContext"/>
        <vae:hasInput rdf:resource="https://w3id.org/def/vaeontology_montes_sierra#jointMoneyTransaction"/>
        <vae:hasInput rdf:resource="https://w3id.org/def/vaeontology_montes_sierra#taxSystemState2"/>
        <vae:hasOutcome rdf:resource="https://w3id.org/def/vaeontology_montes_sierra#taxSystemState3"/>
        <vae:nextInputOutcome rdf:resource="https://w3id.org/def/vaeontology_montes_sierra#path1transition3"/>
    </owl:NamedIndividual>
    


    <!-- https://w3id.org/def/vaeontology_montes_sierra#path1transition3 -->

    <owl:NamedIndividual rdf:about="https://w3id.org/def/vaeontology_montes_sierra#path1transition3">
        <rdf:type rdf:resource="https://w3id.org/def/vaeontology#FinalInputOutcome"/>
        <rdf:type rdf:resource="https://w3id.org/def/vaeontology#Transition"/>
        <dul:hasSetting rdf:resource="https://w3id.org/def/vaeontology_montes_sierra#taxProblemContext"/>
        <vae:hasInput rdf:resource="https://w3id.org/def/vaeontology_montes_sierra#jointMoneyTransaction"/>
        <vae:hasInput rdf:resource="https://w3id.org/def/vaeontology_montes_sierra#taxSystemState3"/>
        <vae:hasOutcome rdf:resource="https://w3id.org/def/vaeontology_montes_sierra#taxSystemState4"/>
    </owl:NamedIndividual>
    


    <!-- https://w3id.org/def/vaeontology_montes_sierra#path2transition1 -->

    <owl:NamedIndividual rdf:about="https://w3id.org/def/vaeontology_montes_sierra#path2transition1">
        <rdf:type rdf:resource="https://w3id.org/def/vaeontology#Transition"/>
        <dul:hasSetting rdf:resource="https://w3id.org/def/vaeontology_montes_sierra#taxProblemContext"/>
        <vae:hasInput rdf:resource="https://w3id.org/def/vaeontology_montes_sierra#jointMoneyTransaction"/>
        <vae:hasInput rdf:resource="https://w3id.org/def/vaeontology_montes_sierra#taxSystemState1"/>
        <vae:hasOutcome rdf:resource="https://w3id.org/def/vaeontology_montes_sierra#taxSystemState3"/>
        <vae:nextInputOutcome rdf:resource="https://w3id.org/def/vaeontology_montes_sierra#path2transition2"/>
    </owl:NamedIndividual>
    


    <!-- https://w3id.org/def/vaeontology_montes_sierra#path2transition2 -->

    <owl:NamedIndividual rdf:about="https://w3id.org/def/vaeontology_montes_sierra#path2transition2">
        <rdf:type rdf:resource="https://w3id.org/def/vaeontology#Transition"/>
        <dul:hasSetting rdf:resource="https://w3id.org/def/vaeontology_montes_sierra#taxProblemContext"/>
        <vae:hasInput rdf:resource="https://w3id.org/def/vaeontology_montes_sierra#jointMoneyTransaction"/>
        <vae:hasInput rdf:resource="https://w3id.org/def/vaeontology_montes_sierra#taxSystemState3"/>
        <vae:hasOutcome rdf:resource="https://w3id.org/def/vaeontology_montes_sierra#taxSystemState2"/>
        <vae:isInputOutcomeOf rdf:resource="https://w3id.org/def/vaeontology_montes_sierra#taxSystemPath2"/>
    </owl:NamedIndividual>
    


    <!-- https://w3id.org/def/vaeontology_montes_sierra#payerAgent1 -->

    <owl:NamedIndividual rdf:about="https://w3id.org/def/vaeontology_montes_sierra#payerAgent1">
        <rdf:type rdf:resource="https://w3id.org/def/vaeontology_montes_sierra#LegalAgent"/>
        <dul:hasSetting rdf:resource="https://w3id.org/def/vaeontology_montes_sierra#taxProblemContext"/>
        <vae:isAgentOfSystem rdf:resource="https://w3id.org/def/vaeontology_montes_sierra#taxingSystem"/>
    </owl:NamedIndividual>
    


    <!-- https://w3id.org/def/vaeontology_montes_sierra#payerAgent1State1 -->

    <owl:NamedIndividual rdf:about="https://w3id.org/def/vaeontology_montes_sierra#payerAgent1State1">
        <rdf:type rdf:resource="https://w3id.org/def/vaeontology_montes_sierra#TaxingAgentState"/>
        <dul:hasSetting rdf:resource="https://w3id.org/def/vaeontology_montes_sierra#taxProblemContext"/>
        <vae:isStateOfAgent rdf:resource="https://w3id.org/def/vaeontology_montes_sierra#payerAgent1"/>
        <belongsToSegment rdf:datatype="http://www.w3.org/2001/XMLSchema#decimal">5</belongsToSegment>
        <hasWealth rdf:datatype="http://www.w3.org/2001/XMLSchema#decimal">99</hasWealth>
    </owl:NamedIndividual>
    


    <!-- https://w3id.org/def/vaeontology_montes_sierra#payerAgent1State2 -->

    <owl:NamedIndividual rdf:about="https://w3id.org/def/vaeontology_montes_sierra#payerAgent1State2">
        <rdf:type rdf:resource="https://w3id.org/def/vaeontology_montes_sierra#TaxingAgentState"/>
        <dul:hasSetting rdf:resource="https://w3id.org/def/vaeontology_montes_sierra#taxProblemContext"/>
        <vae:isStateOfAgent rdf:resource="https://w3id.org/def/vaeontology_montes_sierra#payerAgent1"/>
        <belongsToSegment rdf:datatype="http://www.w3.org/2001/XMLSchema#decimal">3</belongsToSegment>
        <hasWealth rdf:datatype="http://www.w3.org/2001/XMLSchema#decimal">45</hasWealth>
    </owl:NamedIndividual>
    


    <!-- https://w3id.org/def/vaeontology_montes_sierra#payerAgent1State3 -->

    <owl:NamedIndividual rdf:about="https://w3id.org/def/vaeontology_montes_sierra#payerAgent1State3">
        <rdf:type rdf:resource="https://w3id.org/def/vaeontology_montes_sierra#TaxingAgentState"/>
        <dul:hasSetting rdf:resource="https://w3id.org/def/vaeontology_montes_sierra#taxProblemContext"/>
        <vae:isStateOfAgent rdf:resource="https://w3id.org/def/vaeontology_montes_sierra#payerAgent1"/>
        <belongsToSegment rdf:datatype="http://www.w3.org/2001/XMLSchema#decimal">2</belongsToSegment>
        <hasWealth rdf:datatype="http://www.w3.org/2001/XMLSchema#decimal">23</hasWealth>
    </owl:NamedIndividual>
    


    <!-- https://w3id.org/def/vaeontology_montes_sierra#payerAgent1State4 -->

    <owl:NamedIndividual rdf:about="https://w3id.org/def/vaeontology_montes_sierra#payerAgent1State4">
        <rdf:type rdf:resource="https://w3id.org/def/vaeontology_montes_sierra#TaxingAgentState"/>
        <dul:hasSetting rdf:resource="https://w3id.org/def/vaeontology_montes_sierra#taxProblemContext"/>
        <vae:isStateOfAgent rdf:resource="https://w3id.org/def/vaeontology_montes_sierra#payerAgent1"/>
        <belongsToSegment rdf:datatype="http://www.w3.org/2001/XMLSchema#decimal">5</belongsToSegment>
        <hasWealth rdf:datatype="http://www.w3.org/2001/XMLSchema#decimal">87</hasWealth>
    </owl:NamedIndividual>
    


    <!-- https://w3id.org/def/vaeontology_montes_sierra#problemModeller -->

    <owl:NamedIndividual rdf:about="https://w3id.org/def/vaeontology_montes_sierra#problemModeller">
        <rdf:type rdf:resource="https://w3id.org/def/vaeontology#User"/>
        <dul:hasSetting rdf:resource="https://w3id.org/def/vaeontology_montes_sierra#taxProblemContext"/>
        <vae:proposesStatement rdf:resource="https://w3id.org/def/vaeontology_montes_sierra#optimalAlignmentStatementOnNormativeSystemForEquality"/>
        <vae:proposesStatement rdf:resource="https://w3id.org/def/vaeontology_montes_sierra#optimalAlignmentStatementOnNormativeSystemForFairness"/>
    </owl:NamedIndividual>
    


    <!-- https://w3id.org/def/vaeontology_montes_sierra#redistribute -->

    <owl:NamedIndividual rdf:about="https://w3id.org/def/vaeontology_montes_sierra#redistribute">
        <rdf:type rdf:resource="http://www.ontologydesignpatterns.org/ont/dul/DUL.owl#Parameter"/>
        <dul:hasPart rdf:resource="https://w3id.org/def/vaeontology_montes_sierra#redistributeSegment1"/>
        <dul:hasPart rdf:resource="https://w3id.org/def/vaeontology_montes_sierra#redistributeSegment2"/>
        <dul:hasPart rdf:resource="https://w3id.org/def/vaeontology_montes_sierra#redistributeSegment3"/>
        <dul:hasPart rdf:resource="https://w3id.org/def/vaeontology_montes_sierra#redistributeSegment4"/>
        <dul:hasPart rdf:resource="https://w3id.org/def/vaeontology_montes_sierra#redistributeSegment5"/>
        <rdfs:comment>&quot;Table 1: Optimisation results for the running example with respect to the two values of interest plus their aggregation: optimal normative parameters defining the norative system, and their associated optimal alignment.&quot;</rdfs:comment>
    </owl:NamedIndividual>
    


    <!-- https://w3id.org/def/vaeontology_montes_sierra#redistributeF -->

    <owl:NamedIndividual rdf:about="https://w3id.org/def/vaeontology_montes_sierra#redistributeF">
        <rdf:type rdf:resource="http://www.ontologydesignpatterns.org/ont/dul/DUL.owl#Parameter"/>
        <dul:hasPart rdf:resource="https://w3id.org/def/vaeontology_montes_sierra#redistributeFSegment1"/>
        <dul:hasPart rdf:resource="https://w3id.org/def/vaeontology_montes_sierra#redistributeFSegment2"/>
        <dul:hasPart rdf:resource="https://w3id.org/def/vaeontology_montes_sierra#redistributeFSegment3"/>
        <dul:hasPart rdf:resource="https://w3id.org/def/vaeontology_montes_sierra#redistributeFSegment4"/>
        <dul:hasPart rdf:resource="https://w3id.org/def/vaeontology_montes_sierra#redistributeFSegment5"/>
        <rdfs:comment>&quot;Table 1: Optimisation results for the running example with respect to the two values of interest plus their aggregation: optimal normative parameters defining the norative system, and their associated optimal alignment.&quot;</rdfs:comment>
    </owl:NamedIndividual>
    


    <!-- https://w3id.org/def/vaeontology_montes_sierra#redistributeFSegment1 -->

    <owl:NamedIndividual rdf:about="https://w3id.org/def/vaeontology_montes_sierra#redistributeFSegment1">
        <rdf:type rdf:resource="http://www.ontologydesignpatterns.org/ont/dul/DUL.owl#Parameter"/>
        <hasProbabilityOrFraction rdf:datatype="http://www.w3.org/2001/XMLSchema#decimal">0.02</hasProbabilityOrFraction>
        <rdfs:comment>&quot;Table 1: Optimisation results for the running example with respect to the two values of interest plus their aggregation: optimal normative parameters defining the norative system, and their associated optimal alignment.&quot;</rdfs:comment>
    </owl:NamedIndividual>
    


    <!-- https://w3id.org/def/vaeontology_montes_sierra#redistributeFSegment2 -->

    <owl:NamedIndividual rdf:about="https://w3id.org/def/vaeontology_montes_sierra#redistributeFSegment2">
        <rdf:type rdf:resource="http://www.ontologydesignpatterns.org/ont/dul/DUL.owl#Parameter"/>
        <hasProbabilityOrFraction rdf:datatype="http://www.w3.org/2001/XMLSchema#decimal">0.23</hasProbabilityOrFraction>
        <rdfs:comment>&quot;Table 1: Optimisation results for the running example with respect to the two values of interest plus their aggregation: optimal normative parameters defining the norative system, and their associated optimal alignment.&quot;</rdfs:comment>
    </owl:NamedIndividual>
    


    <!-- https://w3id.org/def/vaeontology_montes_sierra#redistributeFSegment3 -->

    <owl:NamedIndividual rdf:about="https://w3id.org/def/vaeontology_montes_sierra#redistributeFSegment3">
        <rdf:type rdf:resource="http://www.ontologydesignpatterns.org/ont/dul/DUL.owl#Parameter"/>
        <hasProbabilityOrFraction rdf:datatype="http://www.w3.org/2001/XMLSchema#decimal">0.42</hasProbabilityOrFraction>
        <rdfs:comment>&quot;Table 1: Optimisation results for the running example with respect to the two values of interest plus their aggregation: optimal normative parameters defining the norative system, and their associated optimal alignment.&quot;</rdfs:comment>
    </owl:NamedIndividual>
    


    <!-- https://w3id.org/def/vaeontology_montes_sierra#redistributeFSegment4 -->

    <owl:NamedIndividual rdf:about="https://w3id.org/def/vaeontology_montes_sierra#redistributeFSegment4">
        <rdf:type rdf:resource="http://www.ontologydesignpatterns.org/ont/dul/DUL.owl#Parameter"/>
        <hasProbabilityOrFraction rdf:datatype="http://www.w3.org/2001/XMLSchema#decimal">0.24</hasProbabilityOrFraction>
        <rdfs:comment>&quot;Table 1: Optimisation results for the running example with respect to the two values of interest plus their aggregation: optimal normative parameters defining the norative system, and their associated optimal alignment.&quot;</rdfs:comment>
    </owl:NamedIndividual>
    


    <!-- https://w3id.org/def/vaeontology_montes_sierra#redistributeFSegment5 -->

    <owl:NamedIndividual rdf:about="https://w3id.org/def/vaeontology_montes_sierra#redistributeFSegment5">
        <rdf:type rdf:resource="http://www.ontologydesignpatterns.org/ont/dul/DUL.owl#Parameter"/>
        <hasProbabilityOrFraction rdf:datatype="http://www.w3.org/2001/XMLSchema#decimal">0.09</hasProbabilityOrFraction>
        <rdfs:comment>&quot;Table 1: Optimisation results for the running example with respect to the two values of interest plus their aggregation: optimal normative parameters defining the norative system, and their associated optimal alignment.&quot;</rdfs:comment>
    </owl:NamedIndividual>
    


    <!-- https://w3id.org/def/vaeontology_montes_sierra#redistributeSegment1 -->

    <owl:NamedIndividual rdf:about="https://w3id.org/def/vaeontology_montes_sierra#redistributeSegment1">
        <rdf:type rdf:resource="http://www.ontologydesignpatterns.org/ont/dul/DUL.owl#Parameter"/>
        <hasProbabilityOrFraction rdf:datatype="http://www.w3.org/2001/XMLSchema#decimal">0.2</hasProbabilityOrFraction>
        <rdfs:comment>&quot;Table 1: Optimisation results for the running example with respect to the two values of interest plus their aggregation: optimal normative parameters defining the norative system, and their associated optimal alignment.&quot;</rdfs:comment>
    </owl:NamedIndividual>
    


    <!-- https://w3id.org/def/vaeontology_montes_sierra#redistributeSegment2 -->

    <owl:NamedIndividual rdf:about="https://w3id.org/def/vaeontology_montes_sierra#redistributeSegment2">
        <rdf:type rdf:resource="http://www.ontologydesignpatterns.org/ont/dul/DUL.owl#Parameter"/>
        <hasProbabilityOrFraction rdf:datatype="http://www.w3.org/2001/XMLSchema#decimal">0.29</hasProbabilityOrFraction>
        <rdfs:comment>&quot;Table 1: Optimisation results for the running example with respect to the two values of interest plus their aggregation: optimal normative parameters defining the norative system, and their associated optimal alignment.&quot;</rdfs:comment>
    </owl:NamedIndividual>
    


    <!-- https://w3id.org/def/vaeontology_montes_sierra#redistributeSegment3 -->

    <owl:NamedIndividual rdf:about="https://w3id.org/def/vaeontology_montes_sierra#redistributeSegment3">
        <rdf:type rdf:resource="http://www.ontologydesignpatterns.org/ont/dul/DUL.owl#Parameter"/>
        <hasProbabilityOrFraction rdf:datatype="http://www.w3.org/2001/XMLSchema#decimal">0.26</hasProbabilityOrFraction>
        <rdfs:comment>&quot;Table 1: Optimisation results for the running example with respect to the two values of interest plus their aggregation: optimal normative parameters defining the norative system, and their associated optimal alignment.&quot;</rdfs:comment>
    </owl:NamedIndividual>
    


    <!-- https://w3id.org/def/vaeontology_montes_sierra#redistributeSegment4 -->

    <owl:NamedIndividual rdf:about="https://w3id.org/def/vaeontology_montes_sierra#redistributeSegment4">
        <rdf:type rdf:resource="http://www.ontologydesignpatterns.org/ont/dul/DUL.owl#Parameter"/>
        <hasProbabilityOrFraction rdf:datatype="http://www.w3.org/2001/XMLSchema#decimal">0.35</hasProbabilityOrFraction>
        <rdfs:comment>&quot;Table 1: Optimisation results for the running example with respect to the two values of interest plus their aggregation: optimal normative parameters defining the norative system, and their associated optimal alignment.&quot;</rdfs:comment>
    </owl:NamedIndividual>
    


    <!-- https://w3id.org/def/vaeontology_montes_sierra#redistributeSegment5 -->

    <owl:NamedIndividual rdf:about="https://w3id.org/def/vaeontology_montes_sierra#redistributeSegment5">
        <rdf:type rdf:resource="http://www.ontologydesignpatterns.org/ont/dul/DUL.owl#Parameter"/>
        <hasProbabilityOrFraction rdf:datatype="http://www.w3.org/2001/XMLSchema#decimal">0.27</hasProbabilityOrFraction>
        <rdfs:comment>&quot;Table 1: Optimisation results for the running example with respect to the two values of interest plus their aggregation: optimal normative parameters defining the norative system, and their associated optimal alignment.&quot;</rdfs:comment>
    </owl:NamedIndividual>
    


    <!-- https://w3id.org/def/vaeontology_montes_sierra#redistribution -->

    <owl:NamedIndividual rdf:about="https://w3id.org/def/vaeontology_montes_sierra#redistribution">
        <rdf:type rdf:resource="https://w3id.org/def/vaeontology#Action"/>
        <dul:hasParticipant rdf:resource="https://w3id.org/def/vaeontology_montes_sierra#evaderAgent1"/>
        <dul:hasParticipant rdf:resource="https://w3id.org/def/vaeontology_montes_sierra#payerAgent1"/>
        <dul:hasSetting rdf:resource="https://w3id.org/def/vaeontology_montes_sierra#taxProblemContext"/>
        <vae:abidesByValue rdf:resource="https://w3id.org/def/vaeontology_montes_sierra#equalityValueTaxing"/>
        <vae:isOutcomeOf rdf:resource="https://w3id.org/def/vaeontology_montes_sierra#path1transition1"/>
        <vae:madeByAgent rdf:resource="https://w3id.org/def/vaeontology_montes_sierra#taxingSystem"/>
    </owl:NamedIndividual>
    


    <!-- https://w3id.org/def/vaeontology_montes_sierra#redistributionStep -->

    <owl:NamedIndividual rdf:about="https://w3id.org/def/vaeontology_montes_sierra#redistributionStep">
        <rdf:type rdf:resource="https://w3id.org/def/vaeontology#FinalInputOutcome"/>
        <vae:hasInput rdf:resource="https://w3id.org/def/vaeontology_montes_sierra#transactionsStep"/>
        <vae:hasOutcome rdf:resource="https://w3id.org/def/vaeontology_montes_sierra#redistribution"/>
        <vae:isInputOutcomeOf rdf:resource="https://w3id.org/def/vaeontology_montes_sierra#taxSystemActionSequence"/>
    </owl:NamedIndividual>
    


    <!-- https://w3id.org/def/vaeontology_montes_sierra#targetPropertyOptimizedAtAction -->

    <owl:NamedIndividual rdf:about="https://w3id.org/def/vaeontology_montes_sierra#targetPropertyOptimizedAtAction">
        <rdf:type rdf:resource="http://www.w3.org/ns/odrl/2/Constraint"/>
        <odrl:leftOperand rdf:resource="https://w3id.org/def/vaeontology_montes_sierra#alignmentPropertyOnNormativeSystemForEquality"/>
        <odrl:operator rdf:resource="https://w3id.org/def/vaeontology_montes_sierra#operatorIsOptimizedAt"/>
        <odrl:rightOperand rdf:resource="https://w3id.org/def/vaeontology_montes_sierra#optimalAlignmentPropertyOnNormativeSystemForEquality"/>
    </owl:NamedIndividual>
    


    <!-- https://w3id.org/def/vaeontology_montes_sierra#taxProblemContext -->

    <owl:NamedIndividual rdf:about="https://w3id.org/def/vaeontology_montes_sierra#taxProblemContext">
        <rdf:type rdf:resource="https://w3id.org/def/vaeontology#Context"/>
    </owl:NamedIndividual>
    


    <!-- https://w3id.org/def/vaeontology_montes_sierra#taxSystemActionSequence -->

    <owl:NamedIndividual rdf:about="https://w3id.org/def/vaeontology_montes_sierra#taxSystemActionSequence">
        <rdf:type rdf:resource="https://w3id.org/def/vaeontology#Sequence"/>
    </owl:NamedIndividual>
    


    <!-- https://w3id.org/def/vaeontology_montes_sierra#taxSystemExecution1 -->

    <owl:NamedIndividual rdf:about="https://w3id.org/def/vaeontology_montes_sierra#taxSystemExecution1">
        <rdf:type rdf:resource="https://w3id.org/def/vaeontology#MultiInputOutcome"/>
        <vae:composedBySequence rdf:resource="https://w3id.org/def/vaeontology_montes_sierra#taxSystemPath1"/>
        <vae:isInputOutcomeOf rdf:resource="https://w3id.org/def/vaeontology_montes_sierra#taxSystemTrace"/>
        <vae:nextInputOutcome rdf:resource="https://w3id.org/def/vaeontology_montes_sierra#taxSystemExecution2"/>
    </owl:NamedIndividual>
    


    <!-- https://w3id.org/def/vaeontology_montes_sierra#taxSystemExecution2 -->

    <owl:NamedIndividual rdf:about="https://w3id.org/def/vaeontology_montes_sierra#taxSystemExecution2">
        <rdf:type rdf:resource="https://w3id.org/def/vaeontology#FinalInputOutcome"/>
        <vae:composedBySequence rdf:resource="https://w3id.org/def/vaeontology_montes_sierra#taxSystemPath2"/>
        <vae:isInputOutcomeOf rdf:resource="https://w3id.org/def/vaeontology_montes_sierra#taxSystemTrace"/>
    </owl:NamedIndividual>
    


    <!-- https://w3id.org/def/vaeontology_montes_sierra#taxSystemPath1 -->

    <owl:NamedIndividual rdf:about="https://w3id.org/def/vaeontology_montes_sierra#taxSystemPath1">
        <rdf:type rdf:resource="https://w3id.org/def/vaeontology#Path"/>
        <dul:hasSetting rdf:resource="https://w3id.org/def/vaeontology_montes_sierra#taxProblemContext"/>
        <vae:abidesByValue rdf:resource="https://w3id.org/def/vaeontology_montes_sierra#equalityValueTaxing"/>
        <vae:abidesByValue rdf:resource="https://w3id.org/def/vaeontology_montes_sierra#fairnessValueTaxing"/>
        <vae:startsWithInputOutcome rdf:resource="https://w3id.org/def/vaeontology_montes_sierra#path1transition1"/>
    </owl:NamedIndividual>
    


    <!-- https://w3id.org/def/vaeontology_montes_sierra#taxSystemPath2 -->

    <owl:NamedIndividual rdf:about="https://w3id.org/def/vaeontology_montes_sierra#taxSystemPath2">
        <rdf:type rdf:resource="https://w3id.org/def/vaeontology#Path"/>
        <dul:hasSetting rdf:resource="https://w3id.org/def/vaeontology_montes_sierra#taxProblemContext"/>
        <vae:abidesByValue rdf:resource="https://w3id.org/def/vaeontology_montes_sierra#equalityValueTaxing"/>
        <vae:abidesByValue rdf:resource="https://w3id.org/def/vaeontology_montes_sierra#fairnessValueTaxing"/>
        <vae:startsWithInputOutcome rdf:resource="https://w3id.org/def/vaeontology_montes_sierra#path2transition1"/>
        <hasOutState rdf:resource="https://w3id.org/def/vaeontology_montes_sierra#taxSystemState2"/>
    </owl:NamedIndividual>
    


    <!-- https://w3id.org/def/vaeontology_montes_sierra#taxSystemState1 -->

    <owl:NamedIndividual rdf:about="https://w3id.org/def/vaeontology_montes_sierra#taxSystemState1">
        <rdf:type rdf:resource="https://w3id.org/def/vaeontology_montes_sierra#TaxingSystemState"/>
        <dul:hasConstituent rdf:resource="https://w3id.org/def/vaeontology_montes_sierra#evaderAgent1State1"/>
        <dul:hasConstituent rdf:resource="https://w3id.org/def/vaeontology_montes_sierra#payerAgent1State1"/>
        <dul:hasSetting rdf:resource="https://w3id.org/def/vaeontology_montes_sierra#taxProblemContext"/>
    </owl:NamedIndividual>
    


    <!-- https://w3id.org/def/vaeontology_montes_sierra#taxSystemState2 -->

    <owl:NamedIndividual rdf:about="https://w3id.org/def/vaeontology_montes_sierra#taxSystemState2">
        <rdf:type rdf:resource="https://w3id.org/def/vaeontology_montes_sierra#TaxingSystemState"/>
        <dul:hasConstituent rdf:resource="https://w3id.org/def/vaeontology_montes_sierra#evaderAgent1State2"/>
        <dul:hasConstituent rdf:resource="https://w3id.org/def/vaeontology_montes_sierra#payerAgent1State2"/>
        <dul:hasSetting rdf:resource="https://w3id.org/def/vaeontology_montes_sierra#taxProblemContext"/>
    </owl:NamedIndividual>
    


    <!-- https://w3id.org/def/vaeontology_montes_sierra#taxSystemState3 -->

    <owl:NamedIndividual rdf:about="https://w3id.org/def/vaeontology_montes_sierra#taxSystemState3">
        <rdf:type rdf:resource="https://w3id.org/def/vaeontology_montes_sierra#TaxingSystemState"/>
        <dul:hasConstituent rdf:resource="https://w3id.org/def/vaeontology_montes_sierra#evaderAgent1State3"/>
        <dul:hasConstituent rdf:resource="https://w3id.org/def/vaeontology_montes_sierra#payerAgent1State3"/>
        <dul:hasSetting rdf:resource="https://w3id.org/def/vaeontology_montes_sierra#taxProblemContext"/>
    </owl:NamedIndividual>
    


    <!-- https://w3id.org/def/vaeontology_montes_sierra#taxSystemState4 -->

    <owl:NamedIndividual rdf:about="https://w3id.org/def/vaeontology_montes_sierra#taxSystemState4">
        <rdf:type rdf:resource="https://w3id.org/def/vaeontology_montes_sierra#TaxingSystemState"/>
        <dul:hasConstituent rdf:resource="https://w3id.org/def/vaeontology_montes_sierra#evaderAgent1State4"/>
        <dul:hasConstituent rdf:resource="https://w3id.org/def/vaeontology_montes_sierra#payerAgent1State4"/>
        <dul:hasSetting rdf:resource="https://w3id.org/def/vaeontology_montes_sierra#taxProblemContext"/>
        <isOutStateOf rdf:resource="https://w3id.org/def/vaeontology_montes_sierra#taxSystemPath1"/>
    </owl:NamedIndividual>
    


    <!-- https://w3id.org/def/vaeontology_montes_sierra#taxSystemTrace -->

    <owl:NamedIndividual rdf:about="https://w3id.org/def/vaeontology_montes_sierra#taxSystemTrace">
        <rdf:type rdf:resource="https://w3id.org/def/vaeontology#Sequence"/>
        <vae:startsWithInputOutcome rdf:resource="https://w3id.org/def/vaeontology_montes_sierra#taxSystemExecution1"/>
    </owl:NamedIndividual>
    


    <!-- https://w3id.org/def/vaeontology_montes_sierra#taxingSystem -->

    <owl:NamedIndividual rdf:about="https://w3id.org/def/vaeontology_montes_sierra#taxingSystem">
        <rdf:type rdf:resource="https://w3id.org/def/vaeontology_montes_sierra#TaxingSystem"/>
        <dul:hasSetting rdf:resource="https://w3id.org/def/vaeontology_montes_sierra#taxProblemContext"/>
        <vae:hasState rdf:resource="https://w3id.org/def/vaeontology_montes_sierra#taxSystemState1"/>
    </owl:NamedIndividual>
    


    <!-- https://w3id.org/def/vaeontology_montes_sierra#transactionNotPayingTaxes -->

    <owl:NamedIndividual rdf:about="https://w3id.org/def/vaeontology_montes_sierra#transactionNotPayingTaxes">
        <rdf:type rdf:resource="https://w3id.org/def/vaeontology_montes_sierra#NotPayingTaxesTransaction"/>
        <dul:hasParticipant rdf:resource="https://w3id.org/def/vaeontology_montes_sierra#payerAgent1"/>
        <dul:hasSetting rdf:resource="https://w3id.org/def/vaeontology_montes_sierra#taxProblemContext"/>
        <vae:madeByAgent rdf:resource="https://w3id.org/def/vaeontology_montes_sierra#evaderAgent1"/>
    </owl:NamedIndividual>
    


    <!-- https://w3id.org/def/vaeontology_montes_sierra#transactionPayingTaxes -->

    <owl:NamedIndividual rdf:about="https://w3id.org/def/vaeontology_montes_sierra#transactionPayingTaxes">
        <rdf:type rdf:resource="https://w3id.org/def/vaeontology_montes_sierra#PayingTaxesTransaction"/>
        <dul:hasParticipant rdf:resource="https://w3id.org/def/vaeontology_montes_sierra#evaderAgent1"/>
        <dul:hasSetting rdf:resource="https://w3id.org/def/vaeontology_montes_sierra#taxProblemContext"/>
        <vae:abidesByValue rdf:resource="https://w3id.org/def/vaeontology_montes_sierra#fairnessValueTaxing"/>
        <vae:madeByAgent rdf:resource="https://w3id.org/def/vaeontology_montes_sierra#payerAgent1"/>
    </owl:NamedIndividual>
    


    <!-- https://w3id.org/def/vaeontology_montes_sierra#transactionsStep -->

    <owl:NamedIndividual rdf:about="https://w3id.org/def/vaeontology_montes_sierra#transactionsStep">
        <rdf:type rdf:resource="https://w3id.org/def/vaeontology#MultiInputOutcome"/>
        <vae:hasOutcome rdf:resource="https://w3id.org/def/vaeontology_montes_sierra#transactionNotPayingTaxes"/>
        <vae:hasOutcome rdf:resource="https://w3id.org/def/vaeontology_montes_sierra#transactionPayingTaxes"/>
        <vae:isStartOfSequence rdf:resource="https://w3id.org/def/vaeontology_montes_sierra#taxSystemActionSequence"/>
        <vae:nextInputOutcome rdf:resource="https://w3id.org/def/vaeontology_montes_sierra#redistributionStep"/>
    </owl:NamedIndividual>
    <rdf:Description>
        <owl:minQualifiedCardinality rdf:datatype="http://www.w3.org/2001/XMLSchema#nonNegativeInteger">1</owl:minQualifiedCardinality>
    </rdf:Description>
</rdf:RDF>



<!-- Generated by the OWL API (version 4.5.26.2023-07-17T20:34:13Z) https://github.com/owlcs/owlapi -->

